separate sim_stutter and sim_nostutter into different files

theories/simulation/slsls.v
@@ -3,45 +3,9 @@
 From iris.bi Require Import bi lib.fixpoint.
 From iris.proofmode Require Import tactics.
 From simuliris.simulation Require Import relations language.
+From simuliris.simulation Require Export simulation.
 From iris.prelude Require Import options.
 Import bi.
-
-Class SimulLang (PROP : bi) (Λ : language) := {
-  (* state interpretation *)
-  state_interp : prog Λ → state Λ → prog Λ → state Λ → PROP;
-  (* value relation that restricts values passed to functions *)
-  val_rel : val Λ → val Λ → PROP;
-}.
-#[global]
-Hint Mode SimulLang + - : typeclass_instances.
-
-Definition progs_are {Λ PROP} `{SimulLang PROP Λ} (P_t P_s : prog Λ) : PROP :=
-  (□ ∀ P_t' P_s' σ_t σ_s, state_interp P_t' σ_t P_s' σ_s → ⌜P_t' = P_t⌝ ∧ ⌜P_s' = P_s⌝)%I.
-#[global]
-Hint Mode progs_are - - - + + : typeclass_instances.
-Typeclasses Opaque progs_are.
-
-Global Instance progs_are_persistent {Λ} {PROP} `{s : SimulLang PROP Λ}
-    (P_s P_t : prog Λ) :
-  Persistent (@progs_are Λ PROP s P_s P_t).
-Proof. rewrite /progs_are; apply _. Qed.
-
-(** Typeclass for the simulation relation so we can use the definitions with
-   greatest+least fp (stuttering) or just greatest fp (no stuttering). *)
-(* TODO: remove this TC once we don't need the no-stutter version anymore*)
-Class Sim {PROP : bi} {Λ : language} (s : SimulLang PROP Λ) :=
-  sim : expr Λ → expr Λ → (val Λ → val Λ → PROP) → PROP.
-#[global]
-Hint Mode Sim - - - : typeclass_instances.
-
-(* FIXME what are good levels for et, es? *)
-Notation "et  '⪯'  es  {{  Φ  }}" := (sim et es Φ) (at level 40, Φ at level 200) : bi_scope.
-(* FIXME: the notation with binder doesn't work; left-factoring seems to fail.
-Notation "et  '⪯'  es  {{  v_t  v_s ,  P  }}" := (sim et es (λ v_t v_s, P)) (at level 40, v_t, v_s at level 200, P at level 200) : bi_scope. *)
-
-(* discrete OFE instance for expr *)
-Definition exprO {Λ : language} := leibnizO (expr Λ).
-Instance expr_equiv {Λ} : Equiv (expr Λ). apply exprO. Defined.
 
 Section fix_lang.
   Context {PROP : bi} `{!BiBUpd PROP, !BiAffine PROP, !BiPureForall PROP}.
@@ -56,878 +20,589 @@ Section fix_lang.
     (σ_s σ_t σ : state Λ)
     (Φ Ψ : val Λ → val Λ → PROP).
 
-  Definition sim_ectx `{!Sim s} K_t K_s Φ :=
-    (∀ v_t v_s, val_rel v_t v_s -∗ sim (fill K_t (of_val v_t)) (fill K_s (of_val v_s)) Φ)%I.
+  (** Simulation relation with stuttering *)
 
-  Section stuttering.
-    (** Simulation relation with stuttering *)
+  Definition least_step Φ (greatest_rec : exprO → exprO → PROP) e_s
+      (least_rec : exprO → PROP) e_t :=
+    (∀ P_t σ_t P_s σ_s, state_interp P_t σ_t P_s σ_s ∗ ⌜¬ reach_stuck P_s e_s σ_s⌝ -∗ |==>
+      (* value case *)
+      (∃ v_t v_s σ_s', ⌜to_val e_t = Some v_t⌝ ∗
+        ⌜rtc (prim_step P_s) (e_s, σ_s) (of_val v_s, σ_s')⌝ ∗
+        state_interp P_t σ_t P_s σ_s' ∗ Φ v_t v_s)
 
-    Definition least_step Φ (greatest_rec : exprO → exprO → PROP) e_s
-        (least_rec : exprO → PROP) e_t :=
-      (∀ P_t σ_t P_s σ_s, state_interp P_t σ_t P_s σ_s ∗ ⌜¬ reach_stuck P_s e_s σ_s⌝ -∗ |==>
-        (* value case *)
-        (∃ v_t v_s σ_s', ⌜to_val e_t = Some v_t⌝ ∗
-          ⌜rtc (prim_step P_s) (e_s, σ_s) (of_val v_s, σ_s')⌝ ∗
-          state_interp P_t σ_t P_s σ_s' ∗ Φ v_t v_s)
+      ∨ (* step case *)
+      (⌜reducible P_t e_t σ_t⌝ ∗ ∀ e_t' σ_t', ⌜prim_step P_t (e_t, σ_t) (e_t', σ_t')⌝ -∗ |==>
+        (* stuttering *)
+        (state_interp P_t σ_t' P_s σ_s ∗ least_rec e_t') ∨
+        (* take a step *)
+        (∃ e_s' σ_s', ⌜tc (prim_step P_s) (e_s, σ_s) (e_s', σ_s')⌝ ∗
+          state_interp P_t σ_t' P_s σ_s' ∗ greatest_rec e_s' e_t'))
 
-        ∨ (* step case *)
-        (⌜reducible P_t e_t σ_t⌝ ∗ ∀ e_t' σ_t', ⌜prim_step P_t (e_t, σ_t) (e_t', σ_t')⌝ -∗ |==>
-          (* stuttering *)
-          (state_interp P_t σ_t' P_s σ_s ∗ least_rec e_t') ∨
-          (* take a step *)
-          (∃ e_s' σ_s', ⌜tc (prim_step P_s) (e_s, σ_s) (e_s', σ_s')⌝ ∗
-            state_interp P_t σ_t' P_s σ_s' ∗ greatest_rec e_s' e_t'))
+      ∨ (* call case *)
+      (∃ f K_t v_t K_s v_s σ_s', ⌜e_t = fill K_t (of_call f v_t)⌝ ∗
+        ⌜rtc (prim_step P_s) (e_s, σ_s) (fill K_s (of_call f v_s), σ_s')⌝ ∗
+        val_rel v_t v_s ∗ state_interp P_t σ_t P_s σ_s' ∗
+        (∀ v_t v_s, val_rel v_t v_s -∗ greatest_rec (fill K_s (of_val v_s)) (fill K_t (of_val v_t))))
+    )%I.
 
-        ∨ (* call case *)
-        (∃ f K_t v_t K_s v_s σ_s', ⌜e_t = fill K_t (of_call f v_t)⌝ ∗
-          ⌜rtc (prim_step P_s) (e_s, σ_s) (fill K_s (of_call f v_s), σ_s')⌝ ∗
-          val_rel v_t v_s ∗ state_interp P_t σ_t P_s σ_s' ∗
-          (∀ v_t v_s, val_rel v_t v_s -∗ greatest_rec (fill K_s (of_val v_s)) (fill K_t (of_val v_t))))
-      )%I.
+  Lemma least_step_mon Φ l1 l2 g1 g2 e_s:
+    ⊢ □ (∀ e, l1 e -∗ l2 e)
+    → □ (∀ e_s e_t, g1 e_s e_t -∗ g2 e_s e_t)
+    → ∀ e, least_step Φ g1 e_s l1 e -∗ least_step Φ g2 e_s l2 e.
+  Proof.
+    iIntros "#H #H0" (e) "Hl". rewrite /least_step. iIntros (P_t σ_t P_s σ_s) "Ha".
+    iMod ("Hl" with "Ha") as "[Hval | [Hstep | Hcall]]"; iModIntro.
+    + iLeft. iApply "Hval".
+    + iRight; iLeft. iDestruct "Hstep" as "[Hred Hr]"; iFrame "Hred".
+      iIntros (e_t' σ_t') "Hstep". iMod ("Hr" with "Hstep") as "[Hstay | Hstep]"; iModIntro.
+      { iLeft. iDestruct "Hstay" as "[$ H1]". by iApply "H". }
+      iRight. iDestruct "Hstep" as (e_s' σ_s') "(H1& H2 &H3)".
+      iExists (e_s'), (σ_s'). iFrame. by iApply "H0".
+    + iRight; iRight. iDestruct "Hcall" as (f K_t v_t K_s v_s σ_s') "(H1& H2& H3& H4&H5)".
+      iExists (f), (K_t), (v_t), (K_s), (v_s), (σ_s'). iFrame.
+      iIntros (? ?) "H1". iApply "H0". by iApply "H5".
+  Qed.
 
-    Lemma least_step_mon Φ l1 l2 g1 g2 e_s:
-      ⊢ □ (∀ e, l1 e -∗ l2 e)
-      → □ (∀ e_s e_t, g1 e_s e_t -∗ g2 e_s e_t)
-      → ∀ e, least_step Φ g1 e_s l1 e -∗ least_step Φ g2 e_s l2 e.
-    Proof.
-      iIntros "#H #H0" (e) "Hl". rewrite /least_step. iIntros (P_t σ_t P_s σ_s) "Ha".
-      iMod ("Hl" with "Ha") as "[Hval | [Hstep | Hcall]]"; iModIntro.
-      + iLeft. iApply "Hval".
-      + iRight; iLeft. iDestruct "Hstep" as "[Hred Hr]"; iFrame "Hred".
-        iIntros (e_t' σ_t') "Hstep". iMod ("Hr" with "Hstep") as "[Hstay | Hstep]"; iModIntro.
-        { iLeft. iDestruct "Hstay" as "[$ H1]". by iApply "H". }
-        iRight. iDestruct "Hstep" as (e_s' σ_s') "(H1& H2 &H3)".
-        iExists (e_s'), (σ_s'). iFrame. by iApply "H0".
-      + iRight; iRight. iDestruct "Hcall" as (f K_t v_t K_s v_s σ_s') "(H1& H2& H3& H4&H5)".
-        iExists (f), (K_t), (v_t), (K_s), (v_s), (σ_s'). iFrame.
-        iIntros (? ?) "H1". iApply "H0". by iApply "H5".
-    Qed.
+  Instance least_step_mono Φ greatest_rec e_s :
+    BiMonoPred (least_step Φ greatest_rec e_s).
+  Proof.
+    constructor.
+    - intros l1 l2. iIntros "H".
+      iApply (least_step_mon Φ l1 l2 greatest_rec greatest_rec e_s with "H").
+      eauto.
+    - intros l Hne n e1 e2 Heq.
+      apply (discrete_iff _ _) in Heq as ->. done.
+  Qed.
 
-    Instance least_step_mono Φ greatest_rec e_s :
-      BiMonoPred (least_step Φ greatest_rec e_s).
-    Proof.
-      constructor.
-      - intros l1 l2. iIntros "H".
-        iApply (least_step_mon Φ l1 l2 greatest_rec greatest_rec e_s with "H").
-        eauto.
-      - intros l Hne n e1 e2 Heq.
-        apply (discrete_iff _ _) in Heq as ->. done.
-    Qed.
+  Definition least_def Φ (greatest_rec : exprO → exprO → PROP) e_s :=
+    bi_least_fixpoint (least_step Φ greatest_rec e_s).
 
-    Definition least_def Φ (greatest_rec : exprO → exprO → PROP) e_s :=
-      bi_least_fixpoint (least_step Φ greatest_rec e_s).
+  Lemma least_def_unfold Φ greatest_rec e_s e_t :
+    least_def Φ greatest_rec e_s e_t ⊣⊢
+      least_step Φ greatest_rec e_s (least_def Φ greatest_rec e_s) e_t.
+  Proof. by rewrite /least_def least_fixpoint_unfold. Qed.
 
-    Lemma least_def_unfold Φ greatest_rec e_s e_t :
-      least_def Φ greatest_rec e_s e_t ⊣⊢
-        least_step Φ greatest_rec e_s (least_def Φ greatest_rec e_s) e_t.
-    Proof. by rewrite /least_def least_fixpoint_unfold. Qed.
+  Definition greatest_step Φ greatest_rec '(e_s, e_t) :=
+    least_def Φ (uncurry greatest_rec) e_s e_t.
 
-    Definition greatest_step Φ greatest_rec '(e_s, e_t) :=
-      least_def Φ (uncurry greatest_rec) e_s e_t.
+  Instance greatest_step_proper Φ greatest_rec :
+    Proper ((≡) ==> (≡)) (greatest_step Φ greatest_rec).
+  Proof. solve_proper. Qed.
 
-    Instance greatest_step_proper Φ greatest_rec :
-      Proper ((≡) ==> (≡)) (greatest_step Φ greatest_rec).
-    Proof. solve_proper. Qed.
+  Lemma least_def_mon Φ g1 g2 e_s:
+    □ (∀ p, g1 p -∗ g2 p) -∗
+    ∀ e, least_def Φ (uncurry g1) e_s e -∗ least_def Φ (uncurry g2) e_s e.
+  Proof.
+    iIntros "#H".
+    rewrite /least_def.
+    iApply (least_fixpoint_ind (least_step Φ (uncurry g1) e_s) (bi_least_fixpoint (least_step Φ (uncurry g2) e_s))).
+    iModIntro. iIntros (e).
+    rewrite least_fixpoint_unfold. iIntros "H0". iApply (least_step_mon Φ _ _ (uncurry g1) (uncurry g2) e_s).
+    - eauto.
+    - iModIntro. iIntros (? ?). rewrite /uncurry. by iApply "H".
+    - iApply "H0".
+  Qed.
 
-    Lemma least_def_mon Φ g1 g2 e_s:
-      □ (∀ p, g1 p -∗ g2 p) -∗
-      ∀ e, least_def Φ (uncurry g1) e_s e -∗ least_def Φ (uncurry g2) e_s e.
-    Proof.
-      iIntros "#H".
-      rewrite /least_def.
-      iApply (least_fixpoint_ind (least_step Φ (uncurry g1) e_s) (bi_least_fixpoint (least_step Φ (uncurry g2) e_s))).
-      iModIntro. iIntros (e).
-      rewrite least_fixpoint_unfold. iIntros "H0". iApply (least_step_mon Φ _ _ (uncurry g1) (uncurry g2) e_s).
-      - eauto.
-      - iModIntro. iIntros (? ?). rewrite /uncurry. by iApply "H".
-      - iApply "H0".
-    Qed.
+  Instance greatest_step_mono Φ :
+    BiMonoPred (greatest_step Φ).
+  Proof.
+    constructor.
+  - intros g1 g2.
+    iIntros "#H" ([e_s e_t]) "Hg". rewrite /greatest_step. iApply least_def_mon; eauto.
+  - intros g Hne n [e_s e_t] [e_s' e_t'] Heq.
+    apply (discrete_iff _ _) in Heq as [-> ->]. done.
+  Qed.
 
-    Instance greatest_step_mono Φ :
-      BiMonoPred (greatest_step Φ).
-    Proof.
-      constructor.
-    - intros g1 g2.
-      iIntros "#H" ([e_s e_t]) "Hg". rewrite /greatest_step. iApply least_def_mon; eauto.
-    - intros g Hne n [e_s e_t] [e_s' e_t'] Heq.
-      apply (discrete_iff _ _) in Heq as [-> ->]. done.
-    Qed.
+  Definition sim_def Φ :=
+    bi_greatest_fixpoint (greatest_step Φ).
 
-    Definition sim_def Φ :=
-      bi_greatest_fixpoint (greatest_step Φ).
+  Lemma sim_def_unfold Φ e_s e_t:
+    sim_def Φ (e_s, e_t) ⊣⊢ greatest_step Φ (sim_def Φ) (e_s, e_t).
+  Proof. by rewrite /sim_def greatest_fixpoint_unfold. Qed.
 
-    Lemma sim_def_unfold Φ e_s e_t:
-      sim_def Φ (e_s, e_t) ⊣⊢ greatest_step Φ (sim_def Φ) (e_s, e_t).
-    Proof. by rewrite /sim_def greatest_fixpoint_unfold. Qed.
+  Lemma sim_def_least_def_unfold Φ e_s e_t :
+    sim_def Φ (e_s, e_t) ⊣⊢ least_def Φ (uncurry (sim_def Φ)) e_s e_t.
+  Proof. by rewrite sim_def_unfold. Qed.
 
-    Lemma sim_def_least_def_unfold Φ e_s e_t :
-      sim_def Φ (e_s, e_t) ⊣⊢ least_def Φ (uncurry (sim_def Φ)) e_s e_t.
-    Proof. by rewrite sim_def_unfold. Qed.
+  Definition sim_aux : seal (λ e_t e_s Φ, @sim_def Φ (e_s, e_t)).
+  Proof. by eexists. Qed.
+  Global Instance sim_stutter : Sim s := sim_aux.(unseal).
+  Lemma sim_eq : sim (Sim:=sim_stutter) = λ e_t e_s Φ, @sim_def Φ (e_s, e_t).
+  Proof. rewrite -sim_aux.(seal_eq) //. Qed.
 
-    Definition sim_aux : seal (λ e_t e_s Φ, @sim_def Φ (e_s, e_t)).
-    Proof. by eexists. Qed.
-    (* Instance is local to avoid ambiguity. *)
-    Instance sim_stutter : Sim s := sim_aux.(unseal).
-    Lemma sim_eq : sim (Sim:=sim_stutter) = λ e_t e_s Φ, @sim_def Φ (e_s, e_t).
-    Proof. rewrite -sim_aux.(seal_eq) //. Qed.
-
-    Lemma sim_unfold Φ e_t e_s:
-      sim (Sim:=sim_stutter) e_t e_s Φ ⊣⊢
-      (∀ P_t σ_t P_s σ_s, state_interp P_t σ_t P_s σ_s ∗ ⌜¬ reach_stuck P_s e_s σ_s⌝ -∗ |==>
-        (* value case *)
-          (∃ v_t v_s σ_s', ⌜to_val e_t = Some v_t⌝ ∗ ⌜rtc (prim_step P_s) (e_s, σ_s) (of_val v_s, σ_s')⌝ ∗
-            state_interp P_t σ_t P_s σ_s' ∗ Φ v_t v_s)
-
-        ∨ (* step case *)
-        (⌜reducible P_t e_t σ_t⌝ ∗ ∀ e_t' σ_t', ⌜prim_step P_t (e_t, σ_t) (e_t', σ_t')⌝ ==∗ 
-          (state_interp P_t σ_t' P_s σ_s ∗ sim e_t' e_s Φ) ∨
-          (∃ e_s' σ_s', ⌜tc (prim_step P_s) (e_s, σ_s) (e_s', σ_s')⌝ ∗ state_interp P_t σ_t' P_s σ_s' ∗
-          sim e_t' e_s' Φ))
-
-        ∨ (* call case *)
-        (∃ f K_t v_t K_s v_s σ_s', ⌜e_t = fill K_t (of_call f v_t)⌝ ∗
-          ⌜rtc (prim_step P_s) (e_s, σ_s) (fill K_s (of_call f v_s), σ_s')⌝ ∗
-          val_rel v_t v_s ∗ state_interp P_t σ_t P_s σ_s' ∗
-          sim_ectx K_t K_s Φ)
-      )%I.
-    Proof.
-      rewrite /sim_ectx !sim_eq /uncurry sim_def_unfold /greatest_step.
-      rewrite least_def_unfold /least_step.
-      setoid_rewrite <-sim_def_least_def_unfold. done.
-    Qed.
-
-    (* any post-fixed point is included in the gfp *)
-    Lemma sim_coind Φ (Ψ : exprO → exprO → PROP) :
-      Proper ((≡) ==> (≡) ==> (≡)) Ψ →
-      ⊢ (□ ∀ e_t e_s, Ψ e_t e_s -∗ greatest_step Φ (λ '(e_s, e_t), Ψ e_t e_s) (e_s, e_t))
-        -∗ ∀ e_t e_s, Ψ e_t e_s -∗ sim e_t e_s Φ.
-    Proof.
-      iIntros (Hp) "#H". iIntros (e_t e_s) "H0".
-      rewrite sim_eq /sim_def.
-
-      set (Ψ_curry := (λ '(e_t, e_s), Ψ e_s e_t)).
-      assert (NonExpansive Ψ_curry) as Hne.
-      { intros ? [e1 e2] [e1' e2'] [H1 H2]. rewrite /Ψ_curry. cbn in H1, H2.
-        apply equiv_dist, Hp.
-        - by apply (discrete_iff _ _) in H1.
-        - by apply (discrete_iff _ _) in H2.
-      }
-      iApply (greatest_fixpoint_coind (greatest_step Φ) Ψ_curry).
-      { iModIntro. iIntros ([e_s' e_t']). iApply "H". }
-      iApply "H0".
-    Qed.
-
-    (* TODO: not sure yet if this lemma is useful. if not, remove *)
-    Lemma sim_strong_ind' e_s Φ (Ψ : exprO → exprO → (val Λ → val Λ → PROP) → PROP):
-      Proper ((≡) ==> (≡) ==> (pointwise_relation (val Λ) (pointwise_relation (val Λ) (≡))) ==> (≡)) Ψ →
-      ⊢ (□ ∀ e_t, least_step Φ (uncurry (sim_def Φ)) e_s
-              (λ e_t', Ψ e_t' e_s Φ ∧ least_def Φ (uncurry (sim_def Φ)) e_s e_t')
-            e_t -∗ Ψ e_t e_s Φ)
-        -∗ ∀ e_t : exprO, (e_t ⪯ e_s {{ Φ }}) -∗ Ψ e_t e_s Φ.
-    Proof.
-      iIntros (Hp) "#IH". iIntros (e_t).
-      rewrite sim_eq /sim_def.
-      rewrite greatest_fixpoint_unfold {2}/greatest_step /least_def.
-
-      change (bi_greatest_fixpoint (greatest_step Φ)) with (sim_def Φ).
-      set (g_rec := least_step Φ (uncurry (sim_def Φ)) e_s).
-
-      set (Ψ' := (λ e_t, Ψ e_t e_s Φ) : exprO → PROP).
-      iAssert ((□ (∀ e_t : exprO, g_rec (λ e_t' : exprO, Ψ' e_t' ∧ bi_least_fixpoint g_rec e_t') e_t -∗ Ψ' e_t)))%I as "#H".
-      { iModIntro. iApply "IH". }
-      iPoseProof (least_fixpoint_strong_ind g_rec Ψ' with "H") as "Htemp".
-      unfold Ψ'. iApply "Htemp".
-    Qed.
-
-    (* TODO: not sure yet if this lemma is useful. if not, remove *)
-    Lemma sim_ind' e_s Φ (Ψ : exprO → exprO → (val Λ → val Λ → PROP) → PROP):
-      Proper ((≡) ==> (≡) ==> (pointwise_relation (val Λ) (pointwise_relation (val Λ) (≡))) ==> (≡)) Ψ →
-      ⊢ (□ ∀ e_t, least_step Φ (uncurry (sim_def Φ)) e_s (λ e_t', Ψ e_t' e_s Φ) e_t -∗ Ψ e_t e_s Φ)
-        -∗ ∀ e_t : exprO, e_t ⪯ e_s {{ Φ }} -∗ Ψ e_t e_s Φ.
-    Proof.
-      iIntros (Hp) "#IH". iApply sim_strong_ind'. iModIntro.
-      iIntros (e_t) "H". iApply "IH".
-      iApply least_step_mon. 3: iApply "H". 2: auto.
-      iModIntro. by iIntros (e) "[H _]".
-    Qed.
-
-    Lemma sim_strong_ind greatest_rec e_s Φ (Ψ : exprO → PROP):
-      Proper ((≡) ==> (≡)) Ψ →
-      (□ ∀ e_t, least_step Φ greatest_rec e_s
-            (λ e_t', Ψ e_t' ∧ least_def Φ greatest_rec e_s e_t')
-        e_t -∗ Ψ e_t) -∗
-      ∀ e_t : exprO, least_def Φ greatest_rec e_s e_t -∗ Ψ e_t.
-    Proof.
-      iIntros (Hp) "#H". iApply least_fixpoint_strong_ind.
-      iModIntro. iIntros (e_t) "IH". by iApply "H".
-    Qed.
-
-    Lemma sim_ind greatest_rec e_s Φ (Ψ : exprO → PROP):
-      Proper ((≡) ==> (≡)) Ψ →
-      (□ ∀ e_t, least_step Φ greatest_rec e_s Ψ e_t -∗ Ψ e_t) -∗
-      ∀ e_t : exprO, least_def Φ greatest_rec e_s e_t -∗ Ψ e_t.
-    Proof.
-      iIntros (Hp) "#H". iApply least_fixpoint_ind.
-      iIntros "!>" (e_t) "IH". by iApply "H".
-    Qed.
-
-    Instance sim_proper :
-      Proper (eq ==> eq ==>
-        (pointwise_relation (val Λ) (pointwise_relation (val Λ) (≡))) ==> (≡)) sim.
-    Proof.
-      intros e e' -> e1 e1' -> p1 p2 Heq2.
-      rewrite !sim_eq. apply greatest_fixpoint_proper; last done.
-      intros p3 [e3 e3']. rewrite /greatest_step /least_def.
-      apply least_fixpoint_proper; last done. solve_proper.
-    Qed.
-
-    Lemma sim_value_target Φ v_t e_s v_s:
-      ⊢ Φ v_t v_s -∗ (∀ P_s σ_s, ⌜rtc (prim_step P_s) (e_s, σ_s) (of_val v_s, σ_s)⌝) -∗ (of_val v_t) ⪯ e_s {{Φ}}.
-    Proof.
-      iIntros "Hv Hr". rewrite sim_unfold. iIntros (????) "[Hstate Hreach]".
-      iModIntro. iLeft. iExists (v_t), (v_s), (σ_s). iFrame.
-      iSplitR; first by rewrite to_of_val. eauto.
-    Qed.
-
-    Lemma sim_value Φ v_t v_s:
-      ⊢ (Φ v_t v_s) -∗ (of_val v_t) ⪯ (of_val v_s) {{ Φ }}.
-    Proof.
-      iIntros "Hv". rewrite sim_unfold. iIntros (????) "[Hstate Hreach]".
-      iModIntro. iLeft. iExists (v_t), (v_s), (σ_s). iFrame.
-      iSplitL; first by rewrite to_of_val. eauto.
-    Qed.
-
-    (* FIXME(RJ) this lemma leaks implementation details? *)
-    Lemma sim_stutter_incl Φ e_s e_t:
-      ⊢ least_def Φ (uncurry (sim_def Φ)) e_s e_t
-        -∗ e_t ⪯ e_s {{ Φ }}.
-    Proof. iIntros "H". by rewrite sim_eq sim_def_unfold /greatest_step. Qed.
-
-    Lemma bupd_sim Φ e_t e_s:
-      ⊢ (|==> e_t ⪯ e_s {{ Φ }}) -∗ e_t ⪯ e_s {{ Φ }}.
-    Proof.
-      iIntros "Hv". rewrite sim_unfold. iIntros (????) "H". iMod "Hv". iApply ("Hv" with "H").
-    Qed.
-
-    Lemma sim_bupd Φ e_t e_s:
-      ⊢ (e_t ⪯ e_s {{ λ v_t v_s, |==> Φ v_t v_s }}) -∗ e_t ⪯ e_s {{ Φ }}.
-    Proof.
-      iIntros "Hv".
-      iApply (sim_coind Φ (λ e_t e_s, e_t ⪯ e_s {{λ v_t v_s, |==> Φ v_t v_s}})%I); last by iFrame.
-      iModIntro. clear e_t e_s. iIntros (e_t e_s) "Hv".
-      rewrite sim_unfold /greatest_step least_def_unfold /least_step.
-      iIntros (????) "H". iMod ("Hv" with "H") as "Hv".
-      iDestruct "Hv" as "[Hv | [H | H]]".
-      - iDestruct "Hv" as (v_t v_s σ_s') "(H1 & H2 & H3 & >H4)".
-        iModIntro. iLeft. iExists v_t, v_s, σ_s'. iFrame.
-      - iModIntro. iRight; iLeft. iDestruct "H" as "[Hred H]"; iFrame.
-        iIntros (??) "Hs". iMod ("H" with "Hs") as "[[? Hs] | Hs]"; iModIntro.
-        + iLeft. iFrame.
-          iApply sim_ind. 2: { rewrite sim_eq sim_def_least_def_unfold. iFrame. }
-          iModIntro. clear e_t' P_t P_s σ_t' σ_t σ_s. iIntros (e_t') "IH".
-          rewrite least_def_unfold !/least_step.
-          iIntros (????) "H". iMod ("IH" with "H") as "Hv".
-          iDestruct "Hv" as "[Hv | [H | H]]".
-          * iDestruct "Hv" as (v_t v_s σ_s') "(H1 & H2 & H3 & >H4)".
-            iModIntro. iLeft. iExists v_t, v_s, σ_s'. iFrame.
-          * iModIntro. iRight; iLeft. iDestruct "H" as "[Hred H]"; iFrame.
-            iIntros (??) "Hs". iMod ("H" with "Hs") as "[[? Hs] | Hs]"; iModIntro.
-            { iLeft. iFrame. }
-            iRight. rewrite sim_eq. iFrame.
-          * iModIntro. iRight; iRight. rewrite sim_eq. iFrame.
-        + iRight. iFrame.
-      - iModIntro. iRight; iRight. iFrame.
-    Qed.
-
-    (* we change the predicate beause at every recursive ocurrence,
-       we give back ownership of the monotonicity assumption *)
-    Lemma least_def_mono rec Φ Φ' :
-      (∀ v_t v_s, Φ v_t v_s -∗ Φ' v_t v_s) -∗
-      ∀ e_s e_t,
-      least_def Φ rec e_s e_t -∗
-      least_def Φ' (λ e_s e_t, rec e_s e_t ∗ ∀ v_t v_s, Φ v_t v_s -∗ Φ' v_t v_s) e_s e_t.
-    Proof.
-      iIntros "Hmon" (e_s e_t). iIntros "Hleast". iRevert "Hmon".
-      iApply (sim_ind _ _ _ (λ e_t, (∀ v_t v_s : val Λ, Φ v_t v_s -∗ Φ' v_t v_s) -∗ least_def Φ' (λ e_s e_t, rec e_s e_t ∗ ∀ v_t v_s, Φ v_t v_s -∗ Φ' v_t v_s) e_s e_t)%I with "[] Hleast"); clear e_t.
-      iModIntro. iIntros (e_t) "IH Hmon". rewrite least_def_unfold /least_step.
-      iIntros (P_t σ_t P_s σ_s) "H". iMod ("IH" with "H") as "IH". iModIntro.
-      iDestruct "IH" as "[Hval | [Hstep | Hcall]]".
-      - iLeft. iDestruct "Hval" as (v_t v_s σ_s') "(?&?&?&?)".
-        iExists v_t, v_s, σ_s'. iFrame. by iApply "Hmon".
-      - iRight; iLeft. iDestruct "Hstep" as "[$ Hstep]".
-        iIntros (e_t' σ_t' Hstep).
-        iMod ("Hstep" with "[//]") as "[Hstep|Hstep]".
-        + iModIntro. iLeft. iDestruct "Hstep" as "[$ H]". by iApply "H".
-        + iModIntro. iRight. iFrame "Hmon". eauto.
-      - iRight; iRight. by iFrame "Hmon".
-    Qed.
-
-    Lemma sim_mono Φ Φ' :
-      (∀ v_t v_s, Φ v_t v_s -∗ Φ' v_t v_s) -∗
-      ∀ e_s e_t : exprO, e_t ⪯ e_s {{ Φ }} -∗ e_t ⪯ e_s {{ Φ' }}.
-    Proof.
-      iIntros "Hmon" (e_s e_t) "H".
-      iApply (sim_coind Φ' (λ e_t e_s, e_t ⪯ e_s {{ Φ }} ∗ (∀ v_t v_s : val Λ, Φ v_t v_s -∗ Φ' v_t v_s))%I); last by iFrame.
-      iModIntro. clear e_t e_s. iIntros (e_t e_s) "[H Hmon]".
-      rewrite sim_eq sim_def_unfold.
-      rewrite /greatest_step !least_def_unfold /least_step.
-      iIntros (????) "Hs". iSpecialize ("H" with "Hs"). iMod "H". iModIntro.
-      iDestruct "H" as "[Hval | [Hred | Hcall]]".
-      - iLeft. iDestruct "Hval" as (v_t v_s σ_s') "(?&?&?&?)".
-        iExists v_t, v_s, σ_s'. iFrame. by iApply "Hmon".
-      - iRight; iLeft. iDestruct "Hred" as "[Hred Hstep]". iFrame.
-        iIntros (e_t' σ_t') "Hprim".
-        iMod ("Hstep" with "Hprim") as "[Hstutter | Hstep]"; iModIntro.
-        + iLeft. iDestruct "Hstutter" as "[Hstate Hleast]". iFrame.
-          by iApply (least_def_mono with "Hmon").
-        + iRight. by iFrame.
-      - iRight; iRight. iFrame.
-    Qed.
-
-    (* TODO: clean up the bind lemma proof *)
-    (* coinduction predicate used for the bind lemma *)
-    Definition bind_pred Φ := uncurry (λ '(e_s, e_t), ∃ e_t' e_s' (K_t K_s : ectx Λ),
-      ⌜e_t = fill K_t e_t'⌝ ∧ ⌜e_s = fill K_s e_s'⌝ ∧
-       e_t' ⪯ e_s' {{ λ v_t v_s : val Λ, fill K_t (of_val v_t) ⪯ fill K_s (of_val v_s) {{ Φ }} }})%I.
-
-    (* Lemma used two times in the proof of the bind lemma (for the value cases of the inner and outer induction) *)
-    Lemma sim_bind_val P_s e_s σ_s v_s σ_s' e_t v_t K_t σ_t P_t K_s Φ:
-        rtc (prim_step P_s) (e_s, σ_s) (of_val v_s, σ_s') →
-        to_val e_t = Some v_t →
-        (¬ reach_stuck P_s (fill K_s e_s) σ_s) →
-        ⊢ fill K_t (of_val v_t) ⪯ fill K_s (of_val v_s) {{Φ}} -∗
-          state_interp P_t σ_t P_s σ_s' -∗ |==>
-
-          (* val case *)
-          (∃ (v_t' v_s' : val Λ) σ_s'', ⌜to_val (fill K_t e_t) = Some v_t'⌝ ∗
-            ⌜rtc (prim_step P_s) (fill K_s e_s, σ_s) (of_val v_s', σ_s'')⌝ ∗
-            state_interp P_t σ_t P_s σ_s'' ∗ Φ v_t' v_s')
-
-          ∨ (* red case *)
-           ⌜reducible P_t (fill K_t e_t) σ_t⌝ ∗
-           (∀ e_t' σ_t',
-              ⌜prim_step P_t (fill K_t e_t, σ_t) (e_t', σ_t')⌝ -∗ |==>
-                (* stutter *)
-                state_interp P_t σ_t' P_s σ_s ∗ least_def Φ (bind_pred Φ) (fill K_s e_s) e_t'
-                ∨ (* step *)
-                (∃ e_s' σ_s'',
-                 ⌜tc (prim_step P_s) (fill K_s e_s, σ_s) (e_s', σ_s'')⌝ ∗ state_interp P_t σ_t' P_s σ_s'' ∗
-                 bind_pred Φ e_s' e_t'))
-          ∨ (* call case *)
-            (∃ (f : string) (K_t' : ectx Λ) (v_t' : val Λ) (K_s' : ectx Λ) (v_s' : val Λ) σ_s'',
-              ⌜fill K_t e_t = fill K_t' (of_call f v_t')⌝ ∗
-              ⌜rtc (prim_step P_s) (fill K_s e_s, σ_s) (fill K_s' (of_call f v_s'), σ_s'')⌝ ∗
-              val_rel v_t' v_s' ∗ state_interp P_t σ_t P_s σ_s'' ∗
-              (∀ v_t'' v_s'' : val Λ, val_rel v_t'' v_s'' -∗
-                bind_pred Φ (fill K_s' (of_val v_s'')) (fill K_t' (of_val v_t'')))).
-    Proof.
-      (* unfold Hpost to examine the result and combine the two simulation proofs *)
-      iIntros (H0 H Hnreach) "Hpost Hstate".
-      rewrite {1}sim_eq {1}sim_def_unfold.
-      rewrite {1}/greatest_step !least_def_unfold /least_step.
-      iMod ("Hpost" with "[Hstate]") as "Hpost".
-      { iFrame. iPureIntro. intros Hstuck. eapply Hnreach, prim_step_rtc_reach_stuck.
-        1:by apply fill_prim_step_rtc. assumption. }
-      iModIntro.
-      iDestruct "Hpost" as "[Hv | [Hstep | Hcall]]".
-      + iLeft. iDestruct "Hv" as (v_t' v_s' σ_s'') "(% & % & Hstate & Hpost)".
-        iExists v_t', v_s', σ_s''. iFrame.
-        iSplitL. { iPureIntro. by rewrite -H1 (of_to_val _ _ H). }
-        iPureIntro. etrans; eauto using fill_prim_step_rtc.
-      + iRight; iLeft. iDestruct "Hstep" as "[% Hstep]". iSplitR "Hstep".
-        { iPureIntro. by rewrite (of_to_val _ _ H) in H1. }
-        iIntros (e_t' σ_t') "%". iMod ("Hstep" with "[]") as "Hstep".
-        { iPureIntro. by rewrite (of_to_val _ _ H). }
-        iModIntro. iDestruct "Hstep" as "[[Hstate Hstutter] | Hstep]".
-        * (* CA on the reduction of e_s to v_s to check if we need to stutter or not *)
-          apply (rtc_inv_tc) in H0 as [Heq | H3].
-          { injection Heq as ??; subst. iLeft. iFrame. iApply least_def_mon. 2: iApply "Hstutter".
-            iModIntro. iIntros ([e_s e_t'']) "H".
-            iExists e_t'', e_s, empty_ectx, empty_ectx.
-            rewrite !fill_empty. do 2 (iSplitR; first auto).
-            iApply sim_mono. 2: { rewrite sim_eq. iApply "H". }
-            iIntros (v_t' v_s') "Hv". rewrite !fill_empty. by iApply sim_value.
-          }
-          {
-            iRight. iExists (fill K_s (of_val v_s)), σ_s'. iFrame.
-            iSplitR "Hstutter".
-            { iPureIntro. by apply fill_prim_step_tc. }
-            cbn. iExists e_t', (fill K_s (of_val v_s)), empty_ectx, empty_ectx. rewrite !fill_empty.
-            do 2 (iSplitR; first auto).
-            iApply sim_mono. 2: { iApply sim_stutter_incl. iApply "Hstutter". }
-            iIntros (v_t' v_s') "Hv". rewrite !fill_empty. by iApply sim_value.
-          }
-        * iDestruct "Hstep" as (e_s' σ_s'') "(%&Hstate& Hrec)". iRight.
-          iExists e_s', σ_s''. iFrame. iSplitR.
-          { iPureIntro. eapply tc_rtc_l; by eauto using fill_prim_step_rtc. }
-          cbn. iExists e_t', e_s', empty_ectx, empty_ectx. rewrite !fill_empty.
-          do 2 (iSplitR; first auto).
-          iApply sim_mono. 2: { rewrite sim_eq. iApply "Hrec". }
-          iIntros (??) "H". rewrite !fill_empty.
-          by iApply sim_value.
-      + iDestruct "Hcall" as (f K_t' v_t' K_s' v_s' σ_s'') "(%&%&Hvrel&Hstate&Hcall)".
-        (* CA on the reduction of fill K_s v_s to fill K_s' (f v_s') to see if we need to take a step or do the call *)
-        iRight; iRight.
-        iExists f, K_t', v_t', K_s', v_s', σ_s''. iFrame.
-        iSplitR. { iPureIntro. by rewrite -H1 (of_to_val _ _ H). }
-        iSplitR. { iPureIntro. etrans; eauto using fill_prim_step_rtc. }
-        iIntros (v_t'' v_s'') "Hvrel". cbn.
-        iExists (fill K_t' (of_val v_t'')), (fill K_s' (of_val v_s'')), empty_ectx, empty_ectx.
-        rewrite !fill_empty. do 2 (iSplitR; first auto).
-        iApply sim_mono; first last.
-        { rewrite sim_eq. by iApply "Hcall". }
-        iIntros (??) "H". rewrite !fill_empty. by iApply sim_value.
-    Qed.
-
-    Lemma sim_bind e_t e_s K_t K_s Φ:
-      ⊢ e_t ⪯ e_s {{λ v_t v_s : val Λ, fill K_t (of_val v_t) ⪯ fill K_s (of_val v_s) {{Φ}} }}
-        -∗ fill K_t e_t ⪯ fill K_s e_s {{Φ}}.
-    Proof.
-      iIntros "H".
-      iApply (sim_coind Φ (λ e_t' e_s', bind_pred Φ e_s' e_t')%I).
-      2: { iExists e_t, e_s, K_t, K_s. iFrame. eauto. }
-      iModIntro. clear e_t e_s K_t K_s.
-      iIntros (e_t' e_s') "IH".
-      iDestruct "IH" as (e_t e_s K_t K_s) "[-> [-> H]]".
-      rewrite {1}sim_eq {1}sim_def_unfold.
-      rewrite /greatest_step !least_def_unfold /least_step.
-
-      iIntros (????) "[Hs %]". rename H into Hnreach.
-      iMod ("H" with "[Hs]") as "H".
-      { iFrame. iPureIntro. contradict Hnreach. by apply fill_reach_stuck. }
-      iDestruct "H" as "[Hval | [Hstep | Hcall]]".
-      - iDestruct "Hval" as (v_t v_s σ_s') "(%& %&Hstate&Hpost)".
-        by iApply (sim_bind_val with "[Hpost] [Hstate]").
-      - (* simply thread through everything *)
-        iModIntro. iRight; iLeft. iDestruct "Hstep" as "[% Hstep]".
-        iSplitR. { iPureIntro. by apply fill_reducible. }
-        iIntros (e_t' σ_t') "%".
-        destruct (fill_reducible_prim_step _ _ _ _ _ _ H H0) as (e_t'' & -> & H1).
-        iMod ("Hstep" with "[]") as "Hstep". { iPureIntro. apply H1. }
-        iModIntro. iDestruct "Hstep" as "[[Hstate Hstutter] | Hstep]".
-        + iLeft. iFrame.
-          (* inner induction *)
-          iApply (sim_ind _ _ _ (λ e_t'', least_def Φ (bind_pred Φ) (fill K_s e_s) (fill K_t e_t''))%I); last done.
-          clear H0 H1 e_t'' H e_t σ_t P_t Hnreach P_s σ_s.
-          iModIntro. iIntros (e_t'') "IH". rewrite least_def_unfold /least_step.
-          iIntros (????) "[Hstate %]". iMod ("IH" with "[Hstate ]") as "IH".
-          { iFrame. iPureIntro. contradict H. by apply fill_reach_stuck. }
-          iDestruct "IH" as "[Hval | [Hred | Hcall]]".
-          * iDestruct "Hval" as (v_t v_s σ_s') "(% & % & Hstate & Hrec)".
-            by iApply (sim_bind_val with "[Hrec] [Hstate]").
-          * iModIntro. iDestruct "Hred" as "[% Hred]". iRight; iLeft. iSplitR.
-            { iPureIntro. by apply fill_reducible. }
-            iIntros (e_t' σ_t'') "%".
-            destruct (fill_reducible_prim_step _ _ _ _ _ _ H0 H1) as (e_t''' & -> & H2).
-            iMod ("Hred" with "[ //]") as "[Hstutter | Hstep]"; iModIntro; first by iLeft.
-            iRight. iDestruct "Hstep" as (e_s' σ_s') "(%&Hstate&Hrec)".
-            iExists (fill K_s e_s'), σ_s'. iFrame. iSplitR.
-            { iPureIntro. by apply fill_prim_step_tc. }
-            cbn. iExists e_t''', e_s', K_t, K_s. do 2 (iSplitR; first auto).
-            by rewrite sim_eq.
-          * iModIntro. iDestruct "Hcall" as (f K_t' v_t K_s' v_s σ_s') "(-> & % & Hv & Hstate & Hcall)".
-            iRight; iRight. iExists f, (comp_ectx K_t K_t'), v_t, (comp_ectx K_s K_s'), v_s, σ_s'.
-            iSplitR. { by rewrite fill_comp. }
-            iSplitR. { iPureIntro. rewrite -fill_comp. by apply fill_prim_step_rtc. }
-            iFrame. iIntros (v_t' v_s') "Hv".
-            cbn. iExists (fill K_t' (of_val v_t')), (fill K_s' (of_val v_s')), K_t, K_s.
-            rewrite !fill_comp. do 2 (iSplitR; first auto).
-            rewrite sim_eq. by iApply "Hcall".
-        + iRight. iDestruct "Hstep" as (e_s' σ_s') "(% & Hstate & Hrec)".
-          iExists (fill K_s e_s'), σ_s'. iFrame. iSplitR.
-          { iPureIntro. by apply fill_prim_step_tc. }
-          cbn. iExists e_t'', e_s', K_t, K_s.
-          do 2 (iSplitR; first auto).
-          rewrite sim_eq. iApply "Hrec".
-      - (* simply thread through everything *)
-        iModIntro. iRight; iRight.
-        iDestruct "Hcall" as (f K_t' v_t K_s' v_s σ_s') "(-> & % & Hval & Hstate & Hrec)".
-        iExists f, (comp_ectx K_t K_t'), v_t, (comp_ectx K_s K_s'), v_s, σ_s'.
-        iSplitR; first by rewrite fill_comp.
-        iSplitR. { iPureIntro. rewrite -fill_comp. by apply fill_prim_step_rtc. }
-        iFrame.
-        iIntros (v_t' v_s') "Hv". iSpecialize ("Hrec" with "Hv"). cbn.
-        iExists (fill K_t' (of_val v_t')), (fill K_s' (of_val v_s')), K_t, K_s.
-        iSplitR; first by rewrite -fill_comp. iSplitR; first by rewrite -fill_comp.
-        rewrite sim_eq. iApply "Hrec".
-    Qed.
-
-    (** Corollaries *)
-    Lemma sim_call_inline P_t P_s v_t v_s K_t K_s f Φ:
-      P_t !! f = Some K_t →
-      P_s !! f = Some K_s →
-      ⊢ progs_are P_t P_s ∗ val_rel v_t v_s ∗ sim_ectx K_t K_s Φ -∗ (of_call f v_t) ⪯ (of_call f v_s) {{Φ}}.
-    Proof.
-      intros Htgt Hsrc. iIntros "(#Prog & Val & Sim)".
-      rewrite sim_unfold. iIntros (P_t' σ_t P_s' σ_s) "[SI %]".
-      iModIntro. iRight. iLeft.
-      rewrite /progs_are; iDestruct ("Prog" with "SI") as "[% %]"; subst P_t' P_s'; iClear "Prog".
-      iSplit.
-      - iPureIntro. eapply head_prim_reducible. eexists _, _. by eapply call_head_step_intro.
-      - iIntros (e_t' σ_t' Hstep). iModIntro.
-       pose proof (prim_step_call_inv P_t empty_ectx f v_t e_t' σ_t σ_t') as (K_t' & Heq & -> & ->);
-        first by rewrite fill_empty.
-        rewrite fill_empty in Hstep. iRight.
-        iExists _, _; iFrame; iSplit.
-        + iPureIntro. eapply tc_once, head_prim_step, call_head_step_intro, Hsrc.
-        + rewrite fill_empty; assert (K_t' = K_t) as -> by naive_solver. iApply ("Sim" with "Val").
-    Qed.
-
-    Lemma sim_frame_r e_t e_s R Φ :
-      e_t ⪯ e_s {{ Φ }} ∗ R ⊢ e_t ⪯ e_s {{λ v_t v_s, Φ v_t v_s ∗ R}}.
-    Proof.
-      iIntros "[Hsim HR]". iApply (sim_mono with "[HR] [Hsim//]"). iIntros (v_t v_s) "H". iFrame.
-    Qed.
-
-    Lemma sim_frame_l e_t e_s R Φ :
-      R ∗ e_t ⪯ e_s {{ Φ }} ⊢ e_t ⪯ e_s {{λ v_t v_s, R ∗ Φ v_t v_s}}.
-    Proof.
-      iIntros "[HR Hsim]". iApply (sim_mono with "[HR] [Hsim//]"). iIntros (v_t v_s) "H". iFrame.
-    Qed.
-
-    Lemma sim_wand e_t e_s Φ Ψ :
-      e_t ⪯ e_s {{ Φ }} -∗ (∀ v_t v_s, Φ v_t v_s -∗ Ψ v_t v_s) -∗ e_t ⪯ e_s {{ Ψ }}.
-    Proof. iIntros "H Hv". iApply (sim_mono with "[Hv//] [H//]"). Qed.
-
-    Lemma sim_wand_l e_t e_s Φ Ψ :
-      (∀ v_t v_s, Φ v_t v_s -∗ Ψ v_t v_s) ∗ e_t ⪯ e_s {{ Φ }} ⊢ e_t ⪯ e_s {{ Ψ }}.
-    Proof. iIntros "[Hv H]". iApply (sim_wand with "[H//] [Hv//]"). Qed.
-
-    Lemma sim_wand_r e_t e_s Φ Ψ :
-      e_t ⪯ e_s {{ Φ }} ∗ (∀ v_t v_s, Φ v_t v_s -∗ Ψ v_t v_s) ⊢ e_t ⪯ e_s {{ Ψ }}.
-    Proof. iIntros "[H Hv]". iApply (sim_wand with "[H//] [Hv//]"). Qed.
-
-    Lemma sim_stutter_source e_t e_s Φ :
-      ⊢ (∀ P_t P_s σ_t σ_s, state_interp P_t σ_t P_s σ_s ==∗
-          ⌜reducible P_t e_t σ_t⌝ ∗
-          ∀ e_t' σ_t', ⌜prim_step P_t (e_t, σ_t) (e_t', σ_t')⌝ ==∗
-            state_interp P_t σ_t' P_s σ_s ∗ e_t' ⪯ e_s {{ Φ }}) -∗
-        e_t ⪯ e_s {{ Φ }}.
-    Proof.
-      iIntros "H". rewrite (sim_unfold Φ e_t e_s). iIntros (????) "[H1 H2]".
-      iMod ("H" with "H1") as "H". iModIntro. iRight; iLeft. iDestruct "H" as "(% & Hnext)".
-      iSplitR. { by iPureIntro. }
-      iIntros (e_t' σ_t') "Hstep". iMod ("Hnext" with "Hstep") as "[Hstate Hsim]".
-      iModIntro. iLeft. iFrame.
-    Qed.
-
-    (* the step case of the simulation relation, but the two cases are combined into an rtc in the source *)
-    Lemma sim_step_target e_t e_s Φ:
-      (∀ P_t P_s σ_t σ_s, state_interp P_t σ_t P_s σ_s ==∗
-        ⌜reducible P_t e_t σ_t⌝ ∗ 
-        ∀ e_t' σ_t',
-          ⌜prim_step P_t (e_t, σ_t) (e_t', σ_t')⌝ ==∗
-            ∃ e_s' σ_s', ⌜rtc (prim_step P_s) (e_s, σ_s) (e_s', σ_s')⌝ ∗
-              state_interp P_t σ_t' P_s σ_s' ∗ e_t' ⪯ e_s' {{ Φ }}) -∗
-      e_t ⪯ e_s {{ Φ }}.
-    Proof.
-      iIntros "H". rewrite (sim_unfold Φ e_t e_s). iIntros (????) "[Hstate %]".
-      iMod ("H" with "Hstate") as "[Hred H]". iModIntro. iRight; iLeft.
-      iFrame. iIntros (e_t' σ_t') "Hstep". iMod ("H" with "Hstep") as "H". iModIntro.
-      iDestruct "H" as (e_s' σ_s') "(%&H2&H3)".
-      apply rtc_inv_tc in H0 as [[= -> ->] | H0].
-      - iLeft. iFrame.
-      - iRight; iExists e_s', σ_s'. iFrame. by iPureIntro.
-    Qed.
-
-    Lemma sim_reach_source_stuck e_t e_s Φ :
-      ⊢ (∀ P_s σ_s P_t σ_t, state_interp P_t σ_t P_s σ_s -∗ ⌜ reach_stuck P_s e_s σ_s ⌝) -∗
-        e_t ⪯ e_s {{ Φ }}.
-    Proof.
-      iIntros "H". rewrite sim_unfold. iIntros (????) "[Hs %]".
-      iDestruct ("H" with "Hs") as "%". exfalso. by apply H.
-    Qed.
-
-    Lemma sim_source_stuck e_t e_s Φ :
-      ⊢ (∀ P_s σ_s P_t σ_t, state_interp P_t σ_t P_s σ_s -∗ ⌜ stuck P_s e_s σ_s ⌝) -∗
-        e_t ⪯ e_s {{ Φ }}.
-    Proof.
-      iIntros "H". iApply sim_reach_source_stuck. iIntros (????) "H0". iDestruct ("H" with "H0") as "%".
-      iPureIntro. exists e_s, σ_s. split; [constructor | assumption].
-    Qed.
-  End stuttering.
-
-  Section no_stuttering.
-    (** Simpler relation without stuttering using just a greatest fp. *)
-
-    Definition step_nostutter Φ (greatest_rec : exprO * exprO → PROP) : exprO * exprO → PROP:=
-      λ '(e_s, e_t), (∀ P_t σ_t P_s σ_s, state_interp P_t σ_t P_s σ_s ∗ ⌜¬ reach_stuck P_s e_s σ_s⌝ -∗ |==>
-        (* value case *)
+  Lemma sim_unfold Φ e_t e_s:
+    sim (Sim:=sim_stutter) e_t e_s Φ ⊣⊢
+    (∀ P_t σ_t P_s σ_s, state_interp P_t σ_t P_s σ_s ∗ ⌜¬ reach_stuck P_s e_s σ_s⌝ -∗ |==>
+      (* value case *)
         (∃ v_t v_s σ_s', ⌜to_val e_t = Some v_t⌝ ∗ ⌜rtc (prim_step P_s) (e_s, σ_s) (of_val v_s, σ_s')⌝ ∗
           state_interp P_t σ_t P_s σ_s' ∗ Φ v_t v_s)
 
-        ∨ (* step case *)
-        (⌜reducible P_t e_t σ_t⌝ ∗ ∀ e_t' σ_t', ⌜prim_step P_t (e_t, σ_t) (e_t', σ_t')⌝ -∗ |==>
-          ∃ e_s' σ_s', ⌜tc (prim_step P_s) (e_s, σ_s) (e_s', σ_s')⌝ ∗ state_interp P_t σ_t' P_s σ_s' ∗ greatest_rec (e_s', e_t'))
+      ∨ (* step case *)
+      (⌜reducible P_t e_t σ_t⌝ ∗ ∀ e_t' σ_t', ⌜prim_step P_t (e_t, σ_t) (e_t', σ_t')⌝ ==∗ 
+        (state_interp P_t σ_t' P_s σ_s ∗ sim e_t' e_s Φ) ∨
+        (∃ e_s' σ_s', ⌜tc (prim_step P_s) (e_s, σ_s) (e_s', σ_s')⌝ ∗ state_interp P_t σ_t' P_s σ_s' ∗
+        sim e_t' e_s' Φ))
 
+      ∨ (* call case *)
+      (∃ f K_t v_t K_s v_s σ_s', ⌜e_t = fill K_t (of_call f v_t)⌝ ∗
+        ⌜rtc (prim_step P_s) (e_s, σ_s) (fill K_s (of_call f v_s), σ_s')⌝ ∗
+        val_rel v_t v_s ∗ state_interp P_t σ_t P_s σ_s' ∗
+        sim_ectx K_t K_s Φ)
+    )%I.
+  Proof.
+    rewrite /sim_ectx !sim_eq /uncurry sim_def_unfold /greatest_step.
+    rewrite least_def_unfold /least_step.
+    setoid_rewrite <-sim_def_least_def_unfold. done.
+  Qed.
+
+  (* any post-fixed point is included in the gfp *)
+  Lemma sim_coind Φ (Ψ : exprO → exprO → PROP) :
+    Proper ((≡) ==> (≡) ==> (≡)) Ψ →
+    ⊢ (□ ∀ e_t e_s, Ψ e_t e_s -∗ greatest_step Φ (λ '(e_s, e_t), Ψ e_t e_s) (e_s, e_t))
+      -∗ ∀ e_t e_s, Ψ e_t e_s -∗ sim e_t e_s Φ.
+  Proof.
+    iIntros (Hp) "#H". iIntros (e_t e_s) "H0".
+    rewrite sim_eq /sim_def.
+
+    set (Ψ_curry := (λ '(e_t, e_s), Ψ e_s e_t)).
+    assert (NonExpansive Ψ_curry) as Hne.
+    { intros ? [e1 e2] [e1' e2'] [H1 H2]. rewrite /Ψ_curry. cbn in H1, H2.
+      apply equiv_dist, Hp.
+      - by apply (discrete_iff _ _) in H1.
+      - by apply (discrete_iff _ _) in H2.
+    }
+    iApply (greatest_fixpoint_coind (greatest_step Φ) Ψ_curry).
+    { iModIntro. iIntros ([e_s' e_t']). iApply "H". }
+    iApply "H0".
+  Qed.
+
+  (* TODO: not sure yet if this lemma is useful. if not, remove *)
+  Lemma sim_strong_ind' e_s Φ (Ψ : exprO → exprO → (val Λ → val Λ → PROP) → PROP):
+    Proper ((≡) ==> (≡) ==> (pointwise_relation (val Λ) (pointwise_relation (val Λ) (≡))) ==> (≡)) Ψ →
+    ⊢ (□ ∀ e_t, least_step Φ (uncurry (sim_def Φ)) e_s
+            (λ e_t', Ψ e_t' e_s Φ ∧ least_def Φ (uncurry (sim_def Φ)) e_s e_t')
+          e_t -∗ Ψ e_t e_s Φ)
+      -∗ ∀ e_t : exprO, (e_t ⪯ e_s {{ Φ }}) -∗ Ψ e_t e_s Φ.
+  Proof.
+    iIntros (Hp) "#IH". iIntros (e_t).
+    rewrite sim_eq /sim_def.
+    rewrite greatest_fixpoint_unfold {2}/greatest_step /least_def.
+
+    change (bi_greatest_fixpoint (greatest_step Φ)) with (sim_def Φ).
+    set (g_rec := least_step Φ (uncurry (sim_def Φ)) e_s).
+
+    set (Ψ' := (λ e_t, Ψ e_t e_s Φ) : exprO → PROP).
+    iAssert ((□ (∀ e_t : exprO, g_rec (λ e_t' : exprO, Ψ' e_t' ∧ bi_least_fixpoint g_rec e_t') e_t -∗ Ψ' e_t)))%I as "#H".
+    { iModIntro. iApply "IH". }
+    iPoseProof (least_fixpoint_strong_ind g_rec Ψ' with "H") as "Htemp".
+    unfold Ψ'. iApply "Htemp".
+  Qed.
+
+  (* TODO: not sure yet if this lemma is useful. if not, remove *)
+  Lemma sim_ind' e_s Φ (Ψ : exprO → exprO → (val Λ → val Λ → PROP) → PROP):
+    Proper ((≡) ==> (≡) ==> (pointwise_relation (val Λ) (pointwise_relation (val Λ) (≡))) ==> (≡)) Ψ →
+    ⊢ (□ ∀ e_t, least_step Φ (uncurry (sim_def Φ)) e_s (λ e_t', Ψ e_t' e_s Φ) e_t -∗ Ψ e_t e_s Φ)
+      -∗ ∀ e_t : exprO, e_t ⪯ e_s {{ Φ }} -∗ Ψ e_t e_s Φ.
+  Proof.
+    iIntros (Hp) "#IH". iApply sim_strong_ind'. iModIntro.
+    iIntros (e_t) "H". iApply "IH".
+    iApply least_step_mon. 3: iApply "H". 2: auto.
+    iModIntro. by iIntros (e) "[H _]".
+  Qed.
+
+  Lemma sim_strong_ind greatest_rec e_s Φ (Ψ : exprO → PROP):
+    Proper ((≡) ==> (≡)) Ψ →
+    (□ ∀ e_t, least_step Φ greatest_rec e_s
+          (λ e_t', Ψ e_t' ∧ least_def Φ greatest_rec e_s e_t')
+      e_t -∗ Ψ e_t) -∗
+    ∀ e_t : exprO, least_def Φ greatest_rec e_s e_t -∗ Ψ e_t.
+  Proof.
+    iIntros (Hp) "#H". iApply least_fixpoint_strong_ind.
+    iModIntro. iIntros (e_t) "IH". by iApply "H".
+  Qed.
+
+  Lemma sim_ind greatest_rec e_s Φ (Ψ : exprO → PROP):
+    Proper ((≡) ==> (≡)) Ψ →
+    (□ ∀ e_t, least_step Φ greatest_rec e_s Ψ e_t -∗ Ψ e_t) -∗
+    ∀ e_t : exprO, least_def Φ greatest_rec e_s e_t -∗ Ψ e_t.
+  Proof.
+    iIntros (Hp) "#H". iApply least_fixpoint_ind.
+    iIntros "!>" (e_t) "IH". by iApply "H".
+  Qed.
+
+  Global Instance sim_proper :
+    Proper (eq ==> eq ==>
+      (pointwise_relation (val Λ) (pointwise_relation (val Λ) (≡))) ==> (≡)) sim.
+  Proof.
+    intros e e' -> e1 e1' -> p1 p2 Heq2.
+    rewrite !sim_eq. apply greatest_fixpoint_proper; last done.
+    intros p3 [e3 e3']. rewrite /greatest_step /least_def.
+    apply least_fixpoint_proper; last done. solve_proper.
+  Qed.
+
+  Lemma sim_value_target Φ v_t e_s v_s:
+    ⊢ Φ v_t v_s -∗ (∀ P_s σ_s, ⌜rtc (prim_step P_s) (e_s, σ_s) (of_val v_s, σ_s)⌝) -∗ (of_val v_t) ⪯ e_s {{Φ}}.
+  Proof.
+    iIntros "Hv Hr". rewrite sim_unfold. iIntros (????) "[Hstate Hreach]".
+    iModIntro. iLeft. iExists (v_t), (v_s), (σ_s). iFrame.
+    iSplitR; first by rewrite to_of_val. eauto.
+  Qed.
+
+  Lemma sim_value Φ v_t v_s:
+    ⊢ (Φ v_t v_s) -∗ (of_val v_t) ⪯ (of_val v_s) {{ Φ }}.
+  Proof.
+    iIntros "Hv". rewrite sim_unfold. iIntros (????) "[Hstate Hreach]".
+    iModIntro. iLeft. iExists (v_t), (v_s), (σ_s). iFrame.
+    iSplitL; first by rewrite to_of_val. eauto.
+  Qed.
+
+  (* FIXME(RJ) this lemma leaks implementation details? *)
+  Lemma sim_stutter_incl Φ e_s e_t:
+    ⊢ least_def Φ (uncurry (sim_def Φ)) e_s e_t
+      -∗ e_t ⪯ e_s {{ Φ }}.
+  Proof. iIntros "H". by rewrite sim_eq sim_def_unfold /greatest_step. Qed.
+
+  Lemma bupd_sim Φ e_t e_s:
+    ⊢ (|==> e_t ⪯ e_s {{ Φ }}) -∗ e_t ⪯ e_s {{ Φ }}.
+  Proof.
+    iIntros "Hv". rewrite sim_unfold. iIntros (????) "H". iMod "Hv". iApply ("Hv" with "H").
+  Qed.
+
+  Lemma sim_bupd Φ e_t e_s:
+    ⊢ (e_t ⪯ e_s {{ λ v_t v_s, |==> Φ v_t v_s }}) -∗ e_t ⪯ e_s {{ Φ }}.
+  Proof.
+    iIntros "Hv".
+    iApply (sim_coind Φ (λ e_t e_s, e_t ⪯ e_s {{λ v_t v_s, |==> Φ v_t v_s}})%I); last by iFrame.
+    iModIntro. clear e_t e_s. iIntros (e_t e_s) "Hv".
+    rewrite sim_unfold /greatest_step least_def_unfold /least_step.
+    iIntros (????) "H". iMod ("Hv" with "H") as "Hv".
+    iDestruct "Hv" as "[Hv | [H | H]]".
+    - iDestruct "Hv" as (v_t v_s σ_s') "(H1 & H2 & H3 & >H4)".
+      iModIntro. iLeft. iExists v_t, v_s, σ_s'. iFrame.
+    - iModIntro. iRight; iLeft. iDestruct "H" as "[Hred H]"; iFrame.
+      iIntros (??) "Hs". iMod ("H" with "Hs") as "[[? Hs] | Hs]"; iModIntro.
+      + iLeft. iFrame.
+        iApply sim_ind. 2: { rewrite sim_eq sim_def_least_def_unfold. iFrame. }
+        iModIntro. clear e_t' P_t P_s σ_t' σ_t σ_s. iIntros (e_t') "IH".
+        rewrite least_def_unfold !/least_step.
+        iIntros (????) "H". iMod ("IH" with "H") as "Hv".
+        iDestruct "Hv" as "[Hv | [H | H]]".
+        * iDestruct "Hv" as (v_t v_s σ_s') "(H1 & H2 & H3 & >H4)".
+          iModIntro. iLeft. iExists v_t, v_s, σ_s'. iFrame.
+        * iModIntro. iRight; iLeft. iDestruct "H" as "[Hred H]"; iFrame.
+          iIntros (??) "Hs". iMod ("H" with "Hs") as "[[? Hs] | Hs]"; iModIntro.
+          { iLeft. iFrame. }
+          iRight. rewrite sim_eq. iFrame.
+        * iModIntro. iRight; iRight. rewrite sim_eq. iFrame.
+      + iRight. iFrame.
+    - iModIntro. iRight; iRight. iFrame.
+  Qed.
+
+  (* we change the predicate beause at every recursive ocurrence,
+     we give back ownership of the monotonicity assumption *)
+  Lemma least_def_mono rec Φ Φ' :
+    (∀ v_t v_s, Φ v_t v_s -∗ Φ' v_t v_s) -∗
+    ∀ e_s e_t,
+    least_def Φ rec e_s e_t -∗
+    least_def Φ' (λ e_s e_t, rec e_s e_t ∗ ∀ v_t v_s, Φ v_t v_s -∗ Φ' v_t v_s) e_s e_t.
+  Proof.
+    iIntros "Hmon" (e_s e_t). iIntros "Hleast". iRevert "Hmon".
+    iApply (sim_ind _ _ _ (λ e_t, (∀ v_t v_s : val Λ, Φ v_t v_s -∗ Φ' v_t v_s) -∗ least_def Φ' (λ e_s e_t, rec e_s e_t ∗ ∀ v_t v_s, Φ v_t v_s -∗ Φ' v_t v_s) e_s e_t)%I with "[] Hleast"); clear e_t.
+    iModIntro. iIntros (e_t) "IH Hmon". rewrite least_def_unfold /least_step.
+    iIntros (P_t σ_t P_s σ_s) "H". iMod ("IH" with "H") as "IH". iModIntro.
+    iDestruct "IH" as "[Hval | [Hstep | Hcall]]".
+    - iLeft. iDestruct "Hval" as (v_t v_s σ_s') "(?&?&?&?)".
+      iExists v_t, v_s, σ_s'. iFrame. by iApply "Hmon".
+    - iRight; iLeft. iDestruct "Hstep" as "[$ Hstep]".
+      iIntros (e_t' σ_t' Hstep).
+      iMod ("Hstep" with "[//]") as "[Hstep|Hstep]".
+      + iModIntro. iLeft. iDestruct "Hstep" as "[$ H]". by iApply "H".
+      + iModIntro. iRight. iFrame "Hmon". eauto.
+    - iRight; iRight. by iFrame "Hmon".
+  Qed.
+
+  Lemma sim_mono Φ Φ' :
+    (∀ v_t v_s, Φ v_t v_s -∗ Φ' v_t v_s) -∗
+    ∀ e_s e_t : exprO, e_t ⪯ e_s {{ Φ }} -∗ e_t ⪯ e_s {{ Φ' }}.
+  Proof.
+    iIntros "Hmon" (e_s e_t) "H".
+    iApply (sim_coind Φ' (λ e_t e_s, e_t ⪯ e_s {{ Φ }} ∗ (∀ v_t v_s : val Λ, Φ v_t v_s -∗ Φ' v_t v_s))%I); last by iFrame.
+    iModIntro. clear e_t e_s. iIntros (e_t e_s) "[H Hmon]".
+    rewrite sim_eq sim_def_unfold.
+    rewrite /greatest_step !least_def_unfold /least_step.
+    iIntros (????) "Hs". iSpecialize ("H" with "Hs"). iMod "H". iModIntro.
+    iDestruct "H" as "[Hval | [Hred | Hcall]]".
+    - iLeft. iDestruct "Hval" as (v_t v_s σ_s') "(?&?&?&?)".
+      iExists v_t, v_s, σ_s'. iFrame. by iApply "Hmon".
+    - iRight; iLeft. iDestruct "Hred" as "[Hred Hstep]". iFrame.
+      iIntros (e_t' σ_t') "Hprim".
+      iMod ("Hstep" with "Hprim") as "[Hstutter | Hstep]"; iModIntro.
+      + iLeft. iDestruct "Hstutter" as "[Hstate Hleast]". iFrame.
+        by iApply (least_def_mono with "Hmon").
+      + iRight. by iFrame.
+    - iRight; iRight. iFrame.
+  Qed.
+
+  (* TODO: clean up the bind lemma proof *)
+  (* coinduction predicate used for the bind lemma *)
+  Definition bind_pred Φ := uncurry (λ '(e_s, e_t), ∃ e_t' e_s' (K_t K_s : ectx Λ),
+    ⌜e_t = fill K_t e_t'⌝ ∧ ⌜e_s = fill K_s e_s'⌝ ∧
+     e_t' ⪯ e_s' {{ λ v_t v_s : val Λ, fill K_t (of_val v_t) ⪯ fill K_s (of_val v_s) {{ Φ }} }})%I.
+
+  (* Lemma used two times in the proof of the bind lemma (for the value cases of the inner and outer induction) *)
+  Lemma sim_bind_val P_s e_s σ_s v_s σ_s' e_t v_t K_t σ_t P_t K_s Φ:
+      rtc (prim_step P_s) (e_s, σ_s) (of_val v_s, σ_s') →
+      to_val e_t = Some v_t →
+      (¬ reach_stuck P_s (fill K_s e_s) σ_s) →
+      ⊢ fill K_t (of_val v_t) ⪯ fill K_s (of_val v_s) {{Φ}} -∗
+        state_interp P_t σ_t P_s σ_s' -∗ |==>
+
+        (* val case *)
+        (∃ (v_t' v_s' : val Λ) σ_s'', ⌜to_val (fill K_t e_t) = Some v_t'⌝ ∗
+          ⌜rtc (prim_step P_s) (fill K_s e_s, σ_s) (of_val v_s', σ_s'')⌝ ∗
+          state_interp P_t σ_t P_s σ_s'' ∗ Φ v_t' v_s')
+
+        ∨ (* red case *)
+         ⌜reducible P_t (fill K_t e_t) σ_t⌝ ∗
+         (∀ e_t' σ_t',
+            ⌜prim_step P_t (fill K_t e_t, σ_t) (e_t', σ_t')⌝ -∗ |==>
+              (* stutter *)
+              state_interp P_t σ_t' P_s σ_s ∗ least_def Φ (bind_pred Φ) (fill K_s e_s) e_t'
+              ∨ (* step *)
+              (∃ e_s' σ_s'',
+               ⌜tc (prim_step P_s) (fill K_s e_s, σ_s) (e_s', σ_s'')⌝ ∗ state_interp P_t σ_t' P_s σ_s'' ∗
+               bind_pred Φ e_s' e_t'))
         ∨ (* call case *)
-        (∃ f K_t v_t K_s v_s σ_s', ⌜e_t = fill K_t (of_call f v_t)⌝ ∗
-          ⌜rtc (prim_step P_s) (e_s, σ_s) (fill K_s (of_call f v_s), σ_s')⌝ ∗
-          val_rel v_t v_s ∗ state_interp P_t σ_t P_s σ_s' ∗
-          (∀ v_t v_s, val_rel v_t v_s -∗ greatest_rec (fill K_s (of_val v_s), fill K_t (of_val v_t))))
-      )%I.
-
-    Definition sim_nostutter_def Φ :=
-      bi_greatest_fixpoint (step_nostutter Φ).
-
-    Instance step_nostutter_proper:
-      Proper ((pointwise_relation (val Λ) (pointwise_relation (val Λ) (≡)))
-        ==> (pointwise_relation _ (≡))
-        ==> (≡) ==> (≡)) (step_nostutter).
-    Proof. solve_proper. Qed.
-
-    Instance step_nostutter_mono Φ:
-      BiMonoPred (step_nostutter Φ).
-    Proof.
-      constructor.
-      - intros g1 g2. iIntros "#H".
-        iIntros ([e_s e_t]) "Hg". rewrite /step_nostutter.
-        iIntros (P_t σ_t P_s σ_s) "Ha".
-        iMod ("Hg" with "Ha") as "[Hval | [Hstep | Hcall]]"; iModIntro.
-        + iLeft. iApply "Hval".
-        + iRight; iLeft. iDestruct "Hstep" as "[Hred Hr]"; iFrame "Hred".
-          iIntros (e_t' σ_t') "Hstep". iMod ("Hr" with "Hstep") as "Hstep"; iModIntro.
-          iDestruct "Hstep" as (e_s' σ_s') "(H1& H2 &H3)".
-          iExists (e_s'), (σ_s'). iFrame. by iApply "H".
-        + iRight; iRight. iDestruct "Hcall" as (f K_t v_t K_s v_s σ_s') "(H1& H2& H3& H4&H5)".
-          iExists (f), (K_t), (v_t), (K_s), (v_s), (σ_s'). iFrame.
-          iIntros (? ?) "H1". iApply "H". by iApply "H5".
-      - intros g Hne n e1 e2 Heq.
-        apply (discrete_iff _ _) in Heq as ->. done.
-    Qed.
-
-    Lemma sim_nostutter_def_unfold Φ e_s e_t:
-      sim_nostutter_def Φ (e_s, e_t) ⊣⊢ step_nostutter Φ (sim_nostutter_def Φ) (e_s, e_t).
-    Proof. by rewrite /sim_nostutter_def greatest_fixpoint_unfold. Qed.
-
-    Definition sim_nostutter_aux : seal (λ e_t e_s Φ, @sim_nostutter_def Φ (e_s, e_t)).
-    Proof. by eexists. Qed.
-    Instance sim_nostutter : Sim s := sim_nostutter_aux.(unseal).
-    Lemma sim_nostutter_eq : sim (Sim:=sim_nostutter) = λ e_t e_s Φ, @sim_nostutter_def Φ (e_s, e_t).
-    Proof. by rewrite <-sim_nostutter_aux.(seal_eq). Qed.
-
-    Lemma sim_nostutter_unfold e_t e_s Φ:
-      sim (Sim:=sim_nostutter) e_t e_s Φ ⊣⊢
-      (∀ P_t σ_t P_s σ_s, state_interp P_t σ_t P_s σ_s ∗ ⌜¬ reach_stuck P_s e_s σ_s⌝ -∗ |==>
-        (* value case *)
-          (∃ v_t v_s σ_s', ⌜to_val e_t = Some v_t⌝ ∗ ⌜rtc (prim_step P_s) (e_s, σ_s) (of_val v_s, σ_s')⌝ ∗
-            state_interp P_t σ_t P_s σ_s' ∗ Φ v_t v_s)
-
-        ∨ (* step case *)
-        (⌜reducible P_t e_t σ_t⌝ ∗ ∀ e_t' σ_t', ⌜prim_step P_t (e_t, σ_t) (e_t', σ_t')⌝ -∗ |==>
-          ∃ e_s' σ_s', ⌜tc (prim_step P_s) (e_s, σ_s) (e_s', σ_s')⌝ ∗ state_interp P_t σ_t' P_s σ_s' ∗
-          sim e_t' e_s' Φ)
-
-        ∨ (* call case *)
-        (∃ f K_t v_t K_s v_s σ_s', ⌜e_t = fill K_t (of_call f v_t)⌝ ∗
-          ⌜rtc (prim_step P_s) (e_s, σ_s) (fill K_s (of_call f v_s), σ_s')⌝ ∗
-          val_rel v_t v_s ∗ state_interp P_t σ_t P_s σ_s' ∗
-          sim_ectx K_t K_s Φ)
-      )%I.
-    Proof.
-      by rewrite /sim_ectx !sim_nostutter_eq /uncurry sim_nostutter_def_unfold /step_nostutter.
-    Qed.
-
-    Lemma sim_nostutter_coind Φ (Ψ : exprO → exprO → PROP):
-      Proper ((≡) ==> (≡) ==> (≡)) Ψ →
-      (□ ∀ e_t e_s, Ψ e_t e_s -∗ step_nostutter Φ (λ '(e_s', e_t'), Ψ e_t' e_s') (e_s, e_t)) -∗
-      (∀ e_t e_s, Ψ e_t e_s -∗ e_t ⪯ e_s {{ Φ }}).
-    Proof.
-      iIntros (Hp) "#IH". iIntros (e_t e_s) "H".
-      rewrite sim_nostutter_eq /sim_nostutter_def.
-      set (Ψ_curry := (λ '(e_t, e_s), Ψ e_s e_t)).
-      assert (NonExpansive Ψ_curry) as Hne.
-      { intros ? [e1 e2] [e1' e2'] [H1 H2]. rewrite /Ψ_curry. cbn in H1, H2.
-        apply equiv_dist, Hp.
-        - by apply (discrete_iff _ _) in H1.
-        - by apply (discrete_iff _ _) in H2.
-      }
-
-      iApply (greatest_fixpoint_coind (step_nostutter Φ) Ψ_curry with "[]").
-      { iModIntro. iIntros ([e_s' e_t']) "H'". by iApply "IH". }
-      iApply "H".
-    Qed.
-
-    Instance sim_nostutter_proper :
-      Proper (eq ==> eq ==>
-        (pointwise_relation (val Λ) (pointwise_relation (val Λ) (≡))) ==> (≡)) sim.
-    Proof.
-      intros e e' -> e1 e1' -> p1 p2 Heq2.
-      rewrite !sim_nostutter_eq. apply greatest_fixpoint_proper; solve_proper.
-    Qed.
-
-    Lemma sim_nostutter_value Φ v_t v_s :
-      ⊢ Φ v_t v_s -∗ (of_val v_t) ⪯ (of_val v_s) {{ Φ }}.
-    Proof.
-      iIntros "Hv". rewrite sim_nostutter_unfold. iIntros (????) "[Hstate Hreach]".
-      iModIntro. iLeft. iExists (v_t), (v_s), (σ_s). iFrame.
-      iSplitL; first by rewrite to_of_val. eauto.
-    Qed.
-
-    Lemma sim_nostutter_call P_t P_s v_t v_s K_t K_s f Φ :
-      P_t !! f = Some K_t →
-      P_s !! f = Some K_s →
-      progs_are P_t P_s -∗
-      val_rel v_t v_s -∗
-      sim_ectx K_t K_s Φ -∗
-      (of_call f v_t) ⪯ (of_call f v_s) {{ Φ }}.
-    Proof.
-      intros Htgt Hsrc. iIntros "#Prog Val Sim".
-      rewrite sim_nostutter_unfold. iIntros (P_t' σ_t P_s' σ_s) "[SI %]".
-      iModIntro. iRight. iLeft.
-      rewrite /progs_are; iDestruct ("Prog" with "SI") as "[% %]"; subst P_t' P_s'; iClear "Prog".
-      iSplit.
-      - iPureIntro. eapply head_prim_reducible. eexists _, _. by eapply call_head_step_intro.
-      - iIntros (e_t' σ_t' Hstep). iModIntro.
-       pose proof (prim_step_call_inv P_t empty_ectx f v_t e_t' σ_t σ_t') as (K_t' & Heq & -> & ->);
-        first by rewrite fill_empty.
-        rewrite fill_empty in Hstep.
-        iExists _, _; iFrame; iSplit.
-        + iPureIntro. eapply tc_once, head_prim_step, call_head_step_intro, Hsrc.
-        + rewrite fill_empty; assert (K_t' = K_t) as -> by naive_solver. iApply ("Sim" with "Val").
-    Qed.
-
-    Lemma bupd_sim_nostutter Φ e_t e_s :
-      ⊢ (|==> e_t ⪯ e_s {{Φ}}) -∗ e_t ⪯ e_s {{ Φ }}.
-    Proof.
-      iIntros "Hv". rewrite sim_nostutter_unfold. iIntros (????) "H". iMod "Hv". iApply ("Hv" with "H").
-    Qed.
-
-    Lemma sim_nostutter_mono Φ Φ' :
-      ⊢ (∀ v_t v_s, Φ v_t v_s -∗ Φ' v_t v_s)
-         -∗ ∀ e_s e_t : exprO, e_t ⪯ e_s {{ Φ }} -∗ e_t ⪯ e_s {{ Φ' }}.
-    Proof.
-      iIntros "Hmon".
-      iIntros (e_s e_t) "H".
-      iApply (sim_nostutter_coind Φ' (λ e_t e_s, e_t ⪯ e_s {{ Φ }} ∗ (∀ v_t v_s : val Λ, Φ v_t v_s -∗ Φ' v_t v_s))%I); last by iFrame.
-      iModIntro. clear e_t e_s. iIntros (e_t e_s) "[H Hpost]".
-      rewrite sim_nostutter_eq sim_nostutter_def_unfold.
-      rewrite /step_nostutter.
-      iIntros (????) "Hs". iSpecialize ("H" with "Hs"). iMod "H". iModIntro.
-      iDestruct "H" as "[Hval | [Hred | Hcall]]".
-      - iLeft. iDestruct "Hval" as (v_t v_s σ_s') "(?&?&?&?)". iExists v_t, v_s, σ_s'. iFrame. by iApply "Hpost".
-      - iRight; iLeft. iDestruct "Hred" as "[Hred Hstep]". iFrame.
-      - iRight; iRight. iFrame.
-    Qed.
-
-    (* TODO: currently just copied and adapted from the full lemma above; we don't need the factorisation for this simpler simulation *)
-    Definition bind_pred_nostutter Φ := uncurry (λ '(e_s, e_t), ∃ e_t' e_s' (K_t K_s : ectx Λ),
-      ⌜e_t = fill K_t e_t'⌝ ∧ ⌜e_s = fill K_s e_s'⌝ ∧
-       e_t' ⪯ e_s' {{λ v_t v_s : val Λ, fill K_t (of_val v_t) ⪯ fill K_s (of_val v_s) {{Φ}}}})%I.
-
-    (* Lemma used two times in the proof of the bind lemma (for the value cases of the inner and outer induction) *)
-    Lemma sim_bind_val_nostutter P_s e_s σ_s v_s σ_s' e_t v_t K_t σ_t P_t K_s Φ:
-        rtc (prim_step P_s) (e_s, σ_s) (of_val v_s, σ_s') →
-        to_val e_t = Some v_t →
-        (¬ reach_stuck P_s (fill K_s e_s) σ_s) →
-        ⊢ fill K_t (of_val v_t) ⪯ fill K_s (of_val v_s) {{Φ}} -∗
-          state_interp P_t σ_t P_s σ_s' -∗ |==>
-
-          (* val case *)
-          (∃ (v_t' v_s' : val Λ) σ_s'', ⌜to_val (fill K_t e_t) = Some v_t'⌝ ∗
-            ⌜rtc (prim_step P_s) (fill K_s e_s, σ_s) (of_val v_s', σ_s'')⌝ ∗
-            state_interp P_t σ_t P_s σ_s'' ∗ Φ v_t' v_s')
-
-          ∨ (* red case *)
-           ⌜reducible P_t (fill K_t e_t) σ_t⌝ ∗
-           (∀ e_t' σ_t',
-              ⌜prim_step P_t (fill K_t e_t, σ_t) (e_t', σ_t')⌝ -∗ |==>
-                (∃ e_s' σ_s'',
-                 ⌜tc (prim_step P_s) (fill K_s e_s, σ_s) (e_s', σ_s'')⌝ ∗ state_interp P_t σ_t' P_s σ_s'' ∗
-                 bind_pred_nostutter Φ e_s' e_t'))
-          ∨ (* call case *)
-            (∃ (f : string) (K_t' : ectx Λ) (v_t' : val Λ) (K_s' : ectx Λ) (v_s' : val Λ) σ_s'',
-              ⌜fill K_t e_t = fill K_t' (of_call f v_t')⌝ ∗
-              ⌜rtc (prim_step P_s) (fill K_s e_s, σ_s) (fill K_s' (of_call f v_s'), σ_s'')⌝ ∗
-              val_rel v_t' v_s' ∗ state_interp P_t σ_t P_s σ_s'' ∗
-              (∀ v_t'' v_s'' : val Λ, val_rel v_t'' v_s'' -∗
-                bind_pred_nostutter Φ (fill K_s' (of_val v_s'')) (fill K_t' (of_val v_t'')))).
-    Proof.
-      (* unfold Hpost to examine the result and combine the two simulation proofs *)
-      iIntros (H0 H Hnreach) "Hpost Hstate".
-      rewrite {1}sim_nostutter_eq {1}sim_nostutter_def_unfold.
-      rewrite {1}/step_nostutter.
-      iMod ("Hpost" with "[Hstate]") as "Hpost".
-      { iFrame. iPureIntro. intros Hstuck.
-        eapply Hnreach, prim_step_rtc_reach_stuck; last done.
-        by apply fill_prim_step_rtc. }
-      iModIntro.
-      iDestruct "Hpost" as "[Hv | [Hstep | Hcall]]".
-      + iLeft. iDestruct "Hv" as (v_t' v_s' σ_s'') "(% & % & Hstate & Hpost)".
-        iExists v_t', v_s', σ_s''. iFrame.
-        iSplitL. { iPureIntro. by rewrite -H1 (of_to_val _ _ H). }
-        iPureIntro. etrans; eauto using fill_prim_step_rtc.
-      + iRight; iLeft. iDestruct "Hstep" as "[% Hstep]". iSplitR "Hstep".
-        { iPureIntro. by rewrite (of_to_val _ _ H) in H1. }
-        iIntros (e_t' σ_t') "%". iMod ("Hstep" with "[]") as "Hstep".
-        { iPureIntro. by rewrite (of_to_val _ _ H). }
-        iDestruct "Hstep" as (e_s' σ_s'') "(%&Hstate& Hrec)".
+          (∃ (f : string) (K_t' : ectx Λ) (v_t' : val Λ) (K_s' : ectx Λ) (v_s' : val Λ) σ_s'',
+            ⌜fill K_t e_t = fill K_t' (of_call f v_t')⌝ ∗
+            ⌜rtc (prim_step P_s) (fill K_s e_s, σ_s) (fill K_s' (of_call f v_s'), σ_s'')⌝ ∗
+            val_rel v_t' v_s' ∗ state_interp P_t σ_t P_s σ_s'' ∗
+            (∀ v_t'' v_s'' : val Λ, val_rel v_t'' v_s'' -∗
+              bind_pred Φ (fill K_s' (of_val v_s'')) (fill K_t' (of_val v_t'')))).
+  Proof.
+    (* unfold Hpost to examine the result and combine the two simulation proofs *)
+    iIntros (H0 H Hnreach) "Hpost Hstate".
+    rewrite {1}sim_eq {1}sim_def_unfold.
+    rewrite {1}/greatest_step !least_def_unfold /least_step.
+    iMod ("Hpost" with "[Hstate]") as "Hpost".
+    { iFrame. iPureIntro. intros Hstuck. eapply Hnreach, prim_step_rtc_reach_stuck.
+      1:by apply fill_prim_step_rtc. assumption. }
+    iModIntro.
+    iDestruct "Hpost" as "[Hv | [Hstep | Hcall]]".
+    + iLeft. iDestruct "Hv" as (v_t' v_s' σ_s'') "(% & % & Hstate & Hpost)".
+      iExists v_t', v_s', σ_s''. iFrame.
+      iSplitL. { iPureIntro. by rewrite -H1 (of_to_val _ _ H). }
+      iPureIntro. etrans; eauto using fill_prim_step_rtc.
+    + iRight; iLeft. iDestruct "Hstep" as "[% Hstep]". iSplitR "Hstep".
+      { iPureIntro. by rewrite (of_to_val _ _ H) in H1. }
+      iIntros (e_t' σ_t') "%". iMod ("Hstep" with "[]") as "Hstep".
+      { iPureIntro. by rewrite (of_to_val _ _ H). }
+      iModIntro. iDestruct "Hstep" as "[[Hstate Hstutter] | Hstep]".
+      * (* CA on the reduction of e_s to v_s to check if we need to stutter or not *)
+        apply (rtc_inv_tc) in H0 as [Heq | H3].
+        { injection Heq as ??; subst. iLeft. iFrame. iApply least_def_mon. 2: iApply "Hstutter".
+          iModIntro. iIntros ([e_s e_t'']) "H".
+          iExists e_t'', e_s, empty_ectx, empty_ectx.
+          rewrite !fill_empty. do 2 (iSplitR; first auto).
+          iApply sim_mono. 2: { rewrite sim_eq. iApply "H". }
+          iIntros (v_t' v_s') "Hv". rewrite !fill_empty. by iApply sim_value.
+        }
+        {
+          iRight. iExists (fill K_s (of_val v_s)), σ_s'. iFrame.
+          iSplitR "Hstutter".
+          { iPureIntro. by apply fill_prim_step_tc. }
+          cbn. iExists e_t', (fill K_s (of_val v_s)), empty_ectx, empty_ectx. rewrite !fill_empty.
+          do 2 (iSplitR; first auto).
+          iApply sim_mono. 2: { iApply sim_stutter_incl. iApply "Hstutter". }
+          iIntros (v_t' v_s') "Hv". rewrite !fill_empty. by iApply sim_value.
+        }
+      * iDestruct "Hstep" as (e_s' σ_s'') "(%&Hstate& Hrec)". iRight.
         iExists e_s', σ_s''. iFrame. iSplitR.
         { iPureIntro. eapply tc_rtc_l; by eauto using fill_prim_step_rtc. }
         cbn. iExists e_t', e_s', empty_ectx, empty_ectx. rewrite !fill_empty.
         do 2 (iSplitR; first auto).
-        iApply sim_nostutter_mono. 2: { rewrite sim_nostutter_eq. iApply "Hrec". }
+        iApply sim_mono. 2: { rewrite sim_eq. iApply "Hrec". }
         iIntros (??) "H". rewrite !fill_empty.
-        by iApply sim_nostutter_value.
-      + iDestruct "Hcall" as (f K_t' v_t' K_s' v_s' σ_s'') "(%&%&Hvrel&Hstate&Hcall)".
-        (* CA on the reduction of fill K_s v_s to fill K_s' (f v_s') to see if we need to take a step or do the call *)
-        iRight; iRight.
-        iExists f, K_t', v_t', K_s', v_s', σ_s''. iFrame.
-        iSplitR. { iPureIntro. by rewrite -H1 (of_to_val _ _ H). }
-        iSplitR. { iPureIntro. etrans; by eauto using fill_prim_step_rtc. }
-        iIntros (v_t'' v_s'') "Hvrel". cbn.
-        iExists (fill K_t' (of_val v_t'')), (fill K_s' (of_val v_s'')), empty_ectx, empty_ectx.
-        rewrite !fill_empty. do 2 (iSplitR; first auto).
-        iApply sim_nostutter_mono; first last.
-        { rewrite sim_nostutter_eq. by iApply "Hcall". }
-        iIntros (??) "H". rewrite !fill_empty. by iApply sim_nostutter_value.
-    Qed.
+        by iApply sim_value.
+    + iDestruct "Hcall" as (f K_t' v_t' K_s' v_s' σ_s'') "(%&%&Hvrel&Hstate&Hcall)".
+      (* CA on the reduction of fill K_s v_s to fill K_s' (f v_s') to see if we need to take a step or do the call *)
+      iRight; iRight.
+      iExists f, K_t', v_t', K_s', v_s', σ_s''. iFrame.
+      iSplitR. { iPureIntro. by rewrite -H1 (of_to_val _ _ H). }
+      iSplitR. { iPureIntro. etrans; eauto using fill_prim_step_rtc. }
+      iIntros (v_t'' v_s'') "Hvrel". cbn.
+      iExists (fill K_t' (of_val v_t'')), (fill K_s' (of_val v_s'')), empty_ectx, empty_ectx.
+      rewrite !fill_empty. do 2 (iSplitR; first auto).
+      iApply sim_mono; first last.
+      { rewrite sim_eq. by iApply "Hcall". }
+      iIntros (??) "H". rewrite !fill_empty. by iApply sim_value.
+  Qed.
 
-    Lemma sim_nostutter_bind e_t e_s K_t K_s Φ:
-      ⊢ e_t ⪯ e_s {{λ v_t v_s : val Λ, fill K_t (of_val v_t) ⪯ fill K_s (of_val v_s) {{Φ}} }}
-        -∗ fill K_t e_t ⪯ fill K_s e_s {{Φ}}.
-    Proof.
-      iIntros "H".
-      iApply (sim_nostutter_coind Φ (λ e_t' e_s', bind_pred_nostutter Φ e_s' e_t')%I).
-      2: { iExists e_t, e_s, K_t, K_s. iFrame. eauto. }
-      iModIntro. clear e_t e_s K_t K_s.
-      iIntros (e_t' e_s') "IH".
-      iDestruct "IH" as (e_t e_s K_t K_s) "[-> [-> H]]".
-      rewrite {1}sim_nostutter_eq {1}sim_nostutter_def_unfold.
-      rewrite /step_nostutter.
+  Lemma sim_bind e_t e_s K_t K_s Φ:
+    ⊢ e_t ⪯ e_s {{λ v_t v_s : val Λ, fill K_t (of_val v_t) ⪯ fill K_s (of_val v_s) {{Φ}} }}
+      -∗ fill K_t e_t ⪯ fill K_s e_s {{Φ}}.
+  Proof.
+    iIntros "H".
+    iApply (sim_coind Φ (λ e_t' e_s', bind_pred Φ e_s' e_t')%I).
+    2: { iExists e_t, e_s, K_t, K_s. iFrame. eauto. }
+    iModIntro. clear e_t e_s K_t K_s.
+    iIntros (e_t' e_s') "IH".
+    iDestruct "IH" as (e_t e_s K_t K_s) "[-> [-> H]]".
+    rewrite {1}sim_eq {1}sim_def_unfold.
+    rewrite /greatest_step !least_def_unfold /least_step.
 
-      iIntros (????) "[Hs %]". rename H into Hnreach.
-      iMod ("H" with "[Hs]") as "H".
-      { iFrame. iPureIntro. contradict Hnreach. by apply fill_reach_stuck. }
-      iDestruct "H" as "[Hval | [Hstep | Hcall]]".
-      - iDestruct "Hval" as (v_t v_s σ_s') "(%& %&Hstate&Hpost)".
-        by iApply (sim_bind_val_nostutter with "[Hpost] [Hstate]").
-      - (* simply thread through everything *)
-        iModIntro. iRight; iLeft. iDestruct "Hstep" as "[% Hstep]".
-        iSplitR. { iPureIntro. by apply fill_reducible. }
-        iIntros (e_t' σ_t') "%".
-        destruct (fill_reducible_prim_step _ _ _ _ _ _ H H0) as (e_t'' & -> & H1).
-        iMod ("Hstep" with "[]") as "Hstep". { iPureIntro. apply H1. }
-        iModIntro.
-        iDestruct "Hstep" as (e_s' σ_s') "(% & Hstate & Hrec)".
+    iIntros (????) "[Hs %]". rename H into Hnreach.
+    iMod ("H" with "[Hs]") as "H".
+    { iFrame. iPureIntro. contradict Hnreach. by apply fill_reach_stuck. }
+    iDestruct "H" as "[Hval | [Hstep | Hcall]]".
+    - iDestruct "Hval" as (v_t v_s σ_s') "(%& %&Hstate&Hpost)".
+      by iApply (sim_bind_val with "[Hpost] [Hstate]").
+    - (* simply thread through everything *)
+      iModIntro. iRight; iLeft. iDestruct "Hstep" as "[% Hstep]".
+      iSplitR. { iPureIntro. by apply fill_reducible. }
+      iIntros (e_t' σ_t') "%".
+      destruct (fill_reducible_prim_step _ _ _ _ _ _ H H0) as (e_t'' & -> & H1).
+      iMod ("Hstep" with "[]") as "Hstep". { iPureIntro. apply H1. }
+      iModIntro. iDestruct "Hstep" as "[[Hstate Hstutter] | Hstep]".
+      + iLeft. iFrame.
+        (* inner induction *)
+        iApply (sim_ind _ _ _ (λ e_t'', least_def Φ (bind_pred Φ) (fill K_s e_s) (fill K_t e_t''))%I); last done.
+        clear H0 H1 e_t'' H e_t σ_t P_t Hnreach P_s σ_s.
+        iModIntro. iIntros (e_t'') "IH". rewrite least_def_unfold /least_step.
+        iIntros (????) "[Hstate %]". iMod ("IH" with "[Hstate ]") as "IH".
+        { iFrame. iPureIntro. contradict H. by apply fill_reach_stuck. }
+        iDestruct "IH" as "[Hval | [Hred | Hcall]]".
+        * iDestruct "Hval" as (v_t v_s σ_s') "(% & % & Hstate & Hrec)".
+          by iApply (sim_bind_val with "[Hrec] [Hstate]").
+        * iModIntro. iDestruct "Hred" as "[% Hred]". iRight; iLeft. iSplitR.
+          { iPureIntro. by apply fill_reducible. }
+          iIntros (e_t' σ_t'') "%".
+          destruct (fill_reducible_prim_step _ _ _ _ _ _ H0 H1) as (e_t''' & -> & H2).
+          iMod ("Hred" with "[ //]") as "[Hstutter | Hstep]"; iModIntro; first by iLeft.
+          iRight. iDestruct "Hstep" as (e_s' σ_s') "(%&Hstate&Hrec)".
+          iExists (fill K_s e_s'), σ_s'. iFrame. iSplitR.
+          { iPureIntro. by apply fill_prim_step_tc. }
+          cbn. iExists e_t''', e_s', K_t, K_s. do 2 (iSplitR; first auto).
+          by rewrite sim_eq.
+        * iModIntro. iDestruct "Hcall" as (f K_t' v_t K_s' v_s σ_s') "(-> & % & Hv & Hstate & Hcall)".
+          iRight; iRight. iExists f, (comp_ectx K_t K_t'), v_t, (comp_ectx K_s K_s'), v_s, σ_s'.
+          iSplitR. { by rewrite fill_comp. }
+          iSplitR. { iPureIntro. rewrite -fill_comp. by apply fill_prim_step_rtc. }
+          iFrame. iIntros (v_t' v_s') "Hv".
+          cbn. iExists (fill K_t' (of_val v_t')), (fill K_s' (of_val v_s')), K_t, K_s.
+          rewrite !fill_comp. do 2 (iSplitR; first auto).
+          rewrite sim_eq. by iApply "Hcall".
+      + iRight. iDestruct "Hstep" as (e_s' σ_s') "(% & Hstate & Hrec)".
         iExists (fill K_s e_s'), σ_s'. iFrame. iSplitR.
         { iPureIntro. by apply fill_prim_step_tc. }
         cbn. iExists e_t'', e_s', K_t, K_s.
         do 2 (iSplitR; first auto).
-        rewrite sim_nostutter_eq. iApply "Hrec".
-      - (* simply thread through everything *)
-        iModIntro. iRight; iRight.
-        iDestruct "Hcall" as (f K_t' v_t K_s' v_s σ_s') "(-> & % & Hval & Hstate & Hrec)".
-        iExists f, (comp_ectx K_t K_t'), v_t, (comp_ectx K_s K_s'), v_s, σ_s'.
-        iSplitR; first by rewrite fill_comp.
-        iSplitR. { iPureIntro. rewrite -fill_comp. by apply fill_prim_step_rtc. }
-        iFrame.
-        iIntros (v_t' v_s') "Hv". iSpecialize ("Hrec" with "Hv"). cbn.
-        iExists (fill K_t' (of_val v_t')), (fill K_s' (of_val v_s')), K_t, K_s.
-        iSplitR; first by rewrite -fill_comp. iSplitR; first by rewrite -fill_comp.
-        rewrite sim_nostutter_eq. iApply "Hrec".
-    Qed.
+        rewrite sim_eq. iApply "Hrec".
+    - (* simply thread through everything *)
+      iModIntro. iRight; iRight.
+      iDestruct "Hcall" as (f K_t' v_t K_s' v_s σ_s') "(-> & % & Hval & Hstate & Hrec)".
+      iExists f, (comp_ectx K_t K_t'), v_t, (comp_ectx K_s K_s'), v_s, σ_s'.
+      iSplitR; first by rewrite fill_comp.
+      iSplitR. { iPureIntro. rewrite -fill_comp. by apply fill_prim_step_rtc. }
+      iFrame.
+      iIntros (v_t' v_s') "Hv". iSpecialize ("Hrec" with "Hv"). cbn.
+      iExists (fill K_t' (of_val v_t')), (fill K_s' (of_val v_s')), K_t, K_s.
+      iSplitR; first by rewrite -fill_comp. iSplitR; first by rewrite -fill_comp.
+      rewrite sim_eq. iApply "Hrec".
+  Qed.
 
-  End no_stuttering.
+  (** Corollaries *)
+  Lemma sim_call_inline P_t P_s v_t v_s K_t K_s f Φ:
+    P_t !! f = Some K_t →
+    P_s !! f = Some K_s →
+    ⊢ progs_are P_t P_s ∗ val_rel v_t v_s ∗ sim_ectx K_t K_s Φ -∗ (of_call f v_t) ⪯ (of_call f v_s) {{Φ}}.
+  Proof.
+    intros Htgt Hsrc. iIntros "(#Prog & Val & Sim)".
+    rewrite sim_unfold. iIntros (P_t' σ_t P_s' σ_s) "[SI %]".
+    iModIntro. iRight. iLeft.
+    rewrite /progs_are; iDestruct ("Prog" with "SI") as "[% %]"; subst P_t' P_s'; iClear "Prog".
+    iSplit.
+    - iPureIntro. eapply head_prim_reducible. eexists _, _. by eapply call_head_step_intro.
+    - iIntros (e_t' σ_t' Hstep). iModIntro.
+     pose proof (prim_step_call_inv P_t empty_ectx f v_t e_t' σ_t σ_t') as (K_t' & Heq & -> & ->);
+      first by rewrite fill_empty.
+      rewrite fill_empty in Hstep. iRight.
+      iExists _, _; iFrame; iSplit.
+      + iPureIntro. eapply tc_once, head_prim_step, call_head_step_intro, Hsrc.
+      + rewrite fill_empty; assert (K_t' = K_t) as -> by naive_solver. iApply ("Sim" with "Val").
+  Qed.
+
+  Lemma sim_frame_r e_t e_s R Φ :
+    e_t ⪯ e_s {{ Φ }} ∗ R ⊢ e_t ⪯ e_s {{λ v_t v_s, Φ v_t v_s ∗ R}}.
+  Proof.
+    iIntros "[Hsim HR]". iApply (sim_mono with "[HR] [Hsim//]"). iIntros (v_t v_s) "H". iFrame.
+  Qed.
+
+  Lemma sim_frame_l e_t e_s R Φ :
+    R ∗ e_t ⪯ e_s {{ Φ }} ⊢ e_t ⪯ e_s {{λ v_t v_s, R ∗ Φ v_t v_s}}.
+  Proof.
+    iIntros "[HR Hsim]". iApply (sim_mono with "[HR] [Hsim//]"). iIntros (v_t v_s) "H". iFrame.
+  Qed.
+
+  Lemma sim_wand e_t e_s Φ Ψ :
+    e_t ⪯ e_s {{ Φ }} -∗ (∀ v_t v_s, Φ v_t v_s -∗ Ψ v_t v_s) -∗ e_t ⪯ e_s {{ Ψ }}.
+  Proof. iIntros "H Hv". iApply (sim_mono with "[Hv//] [H//]"). Qed.
+
+  Lemma sim_wand_l e_t e_s Φ Ψ :
+    (∀ v_t v_s, Φ v_t v_s -∗ Ψ v_t v_s) ∗ e_t ⪯ e_s {{ Φ }} ⊢ e_t ⪯ e_s {{ Ψ }}.
+  Proof. iIntros "[Hv H]". iApply (sim_wand with "[H//] [Hv//]"). Qed.
+
+  Lemma sim_wand_r e_t e_s Φ Ψ :
+    e_t ⪯ e_s {{ Φ }} ∗ (∀ v_t v_s, Φ v_t v_s -∗ Ψ v_t v_s) ⊢ e_t ⪯ e_s {{ Ψ }}.
+  Proof. iIntros "[H Hv]". iApply (sim_wand with "[H//] [Hv//]"). Qed.
+
+  Lemma sim_stutter_source e_t e_s Φ :
+    ⊢ (∀ P_t P_s σ_t σ_s, state_interp P_t σ_t P_s σ_s ==∗
+        ⌜reducible P_t e_t σ_t⌝ ∗
+        ∀ e_t' σ_t', ⌜prim_step P_t (e_t, σ_t) (e_t', σ_t')⌝ ==∗
+          state_interp P_t σ_t' P_s σ_s ∗ e_t' ⪯ e_s {{ Φ }}) -∗
+      e_t ⪯ e_s {{ Φ }}.
+  Proof.
+    iIntros "H". rewrite (sim_unfold Φ e_t e_s). iIntros (????) "[H1 H2]".
+    iMod ("H" with "H1") as "H". iModIntro. iRight; iLeft. iDestruct "H" as "(% & Hnext)".
+    iSplitR. { by iPureIntro. }
+    iIntros (e_t' σ_t') "Hstep". iMod ("Hnext" with "Hstep") as "[Hstate Hsim]".
+    iModIntro. iLeft. iFrame.
+  Qed.
+
+  (* the step case of the simulation relation, but the two cases are combined into an rtc in the source *)
+  Lemma sim_step_target e_t e_s Φ:
+    (∀ P_t P_s σ_t σ_s, state_interp P_t σ_t P_s σ_s ==∗
+      ⌜reducible P_t e_t σ_t⌝ ∗ 
+      ∀ e_t' σ_t',
+        ⌜prim_step P_t (e_t, σ_t) (e_t', σ_t')⌝ ==∗
+          ∃ e_s' σ_s', ⌜rtc (prim_step P_s) (e_s, σ_s) (e_s', σ_s')⌝ ∗
+            state_interp P_t σ_t' P_s σ_s' ∗ e_t' ⪯ e_s' {{ Φ }}) -∗
+    e_t ⪯ e_s {{ Φ }}.
+  Proof.
+    iIntros "H". rewrite (sim_unfold Φ e_t e_s). iIntros (????) "[Hstate %]".
+    iMod ("H" with "Hstate") as "[Hred H]". iModIntro. iRight; iLeft.
+    iFrame. iIntros (e_t' σ_t') "Hstep". iMod ("H" with "Hstep") as "H". iModIntro.
+    iDestruct "H" as (e_s' σ_s') "(%&H2&H3)".
+    apply rtc_inv_tc in H0 as [[= -> ->] | H0].
+    - iLeft. iFrame.
+    - iRight; iExists e_s', σ_s'. iFrame. by iPureIntro.
+  Qed.
+
+  Lemma sim_reach_source_stuck e_t e_s Φ :
+    ⊢ (∀ P_s σ_s P_t σ_t, state_interp P_t σ_t P_s σ_s -∗ ⌜ reach_stuck P_s e_s σ_s ⌝) -∗
+      e_t ⪯ e_s {{ Φ }}.
+  Proof.
+    iIntros "H". rewrite sim_unfold. iIntros (????) "[Hs %]".
+    iDestruct ("H" with "Hs") as "%". exfalso. by apply H.
+  Qed.
+
+  Lemma sim_source_stuck e_t e_s Φ :
+    ⊢ (∀ P_s σ_s P_t σ_t, state_interp P_t σ_t P_s σ_s -∗ ⌜ stuck P_s e_s σ_s ⌝) -∗
+      e_t ⪯ e_s {{ Φ }}.
+  Proof.
+    iIntros "H". iApply sim_reach_source_stuck. iIntros (????) "H0". iDestruct ("H" with "H0") as "%".
+    iPureIntro. exists e_s, σ_s. split; [constructor | assumption].
+  Qed.
 End fix_lang.
 
