theories/simulation/slsls_nostutter.v
@@ -1,0 +1,303 @@
+(** * Simpler relation without stuttering using just a greatest fp. *)
+From iris.bi Require Import bi lib.fixpoint.
+From iris.proofmode Require Import tactics.
+From simuliris.simulation Require Import relations language.
+From simuliris.simulation Require Export simulation.
+From iris.prelude Require Import options.
+Import bi.
+
+Section fix_lang.
+  Context {PROP : bi} `{!BiBUpd PROP, !BiAffine PROP, !BiPureForall PROP}.
+  Context {Λ : language}.
+  Context {s : SimulLang PROP Λ}.
+
+  Set Default Proof Using "Type*".
+
+  Implicit Types
+    (e_s e_t e: expr Λ)
+    (P_s P_t P: prog Λ)
+    (σ_s σ_t σ : state Λ)
+    (Φ Ψ : val Λ → val Λ → PROP).
+
+
+  Definition step_nostutter Φ (greatest_rec : exprO * exprO → PROP) : exprO * exprO → PROP:=
+    λ '(e_s, e_t), (∀ P_t σ_t P_s σ_s, state_interp P_t σ_t P_s σ_s ∗ ⌜¬ reach_stuck P_s e_s σ_s⌝ -∗ |==>
+      (* value case *)
+      (∃ v_t v_s σ_s', ⌜to_val e_t = Some v_t⌝ ∗ ⌜rtc (prim_step P_s) (e_s, σ_s) (of_val v_s, σ_s')⌝ ∗
+        state_interp P_t σ_t P_s σ_s' ∗ Φ v_t v_s)
+
+      ∨ (* step case *)
+      (⌜reducible P_t e_t σ_t⌝ ∗ ∀ e_t' σ_t', ⌜prim_step P_t (e_t, σ_t) (e_t', σ_t')⌝ -∗ |==>
+        ∃ e_s' σ_s', ⌜tc (prim_step P_s) (e_s, σ_s) (e_s', σ_s')⌝ ∗ state_interp P_t σ_t' P_s σ_s' ∗ 
+          greatest_rec (e_s', e_t'))
+
+      ∨ (* call case *)
+      (∃ f K_t v_t K_s v_s σ_s', ⌜e_t = fill K_t (of_call f v_t)⌝ ∗
+        ⌜rtc (prim_step P_s) (e_s, σ_s) (fill K_s (of_call f v_s), σ_s')⌝ ∗
+        val_rel v_t v_s ∗ state_interp P_t σ_t P_s σ_s' ∗
+        (∀ v_t v_s, val_rel v_t v_s -∗ greatest_rec (fill K_s (of_val v_s), fill K_t (of_val v_t))))
+    )%I.
+
+  Definition sim_nostutter_def Φ :=
+    bi_greatest_fixpoint (step_nostutter Φ).
+
+  Instance step_nostutter_proper:
+    Proper ((pointwise_relation (val Λ) (pointwise_relation (val Λ) (≡)))
+      ==> (pointwise_relation _ (≡))
+      ==> (≡) ==> (≡)) (step_nostutter).
+  Proof. solve_proper. Qed.
+
+  Instance step_nostutter_mono Φ:
+    BiMonoPred (step_nostutter Φ).
+  Proof.
+    constructor.
+    - intros g1 g2. iIntros "#H".
+      iIntros ([e_s e_t]) "Hg". rewrite /step_nostutter.
+      iIntros (P_t σ_t P_s σ_s) "Ha".
+      iMod ("Hg" with "Ha") as "[Hval | [Hstep | Hcall]]"; iModIntro.
+      + iLeft. iApply "Hval".
+      + iRight; iLeft. iDestruct "Hstep" as "[Hred Hr]"; iFrame "Hred".
+        iIntros (e_t' σ_t') "Hstep". iMod ("Hr" with "Hstep") as "Hstep"; iModIntro.
+        iDestruct "Hstep" as (e_s' σ_s') "(H1& H2 &H3)".
+        iExists (e_s'), (σ_s'). iFrame. by iApply "H".
+      + iRight; iRight. iDestruct "Hcall" as (f K_t v_t K_s v_s σ_s') "(H1& H2& H3& H4&H5)".
+        iExists (f), (K_t), (v_t), (K_s), (v_s), (σ_s'). iFrame.
+        iIntros (? ?) "H1". iApply "H". by iApply "H5".
+    - intros g Hne n e1 e2 Heq.
+      apply (discrete_iff _ _) in Heq as ->. done.
+  Qed.
+
+  Lemma sim_nostutter_def_unfold Φ e_s e_t:
+    sim_nostutter_def Φ (e_s, e_t) ⊣⊢ step_nostutter Φ (sim_nostutter_def Φ) (e_s, e_t).
+  Proof. by rewrite /sim_nostutter_def greatest_fixpoint_unfold. Qed.
+
+  Definition sim_nostutter_aux : seal (λ e_t e_s Φ, @sim_nostutter_def Φ (e_s, e_t)).
+  Proof. by eexists. Qed.
+  Global Instance sim_nostutter : Sim s := sim_nostutter_aux.(unseal).
+  Lemma sim_nostutter_eq : sim (Sim:=sim_nostutter) = λ e_t e_s Φ, @sim_nostutter_def Φ (e_s, e_t).
+  Proof. by rewrite <-sim_nostutter_aux.(seal_eq). Qed.
+
+  Lemma sim_nostutter_unfold e_t e_s Φ:
+    sim (Sim:=sim_nostutter) e_t e_s Φ ⊣⊢
+    (∀ P_t σ_t P_s σ_s, state_interp P_t σ_t P_s σ_s ∗ ⌜¬ reach_stuck P_s e_s σ_s⌝ -∗ |==>
+      (* value case *)
+        (∃ v_t v_s σ_s', ⌜to_val e_t = Some v_t⌝ ∗ ⌜rtc (prim_step P_s) (e_s, σ_s) (of_val v_s, σ_s')⌝ ∗
+          state_interp P_t σ_t P_s σ_s' ∗ Φ v_t v_s)
+
+      ∨ (* step case *)
+      (⌜reducible P_t e_t σ_t⌝ ∗ ∀ e_t' σ_t', ⌜prim_step P_t (e_t, σ_t) (e_t', σ_t')⌝ -∗ |==>
+        ∃ e_s' σ_s', ⌜tc (prim_step P_s) (e_s, σ_s) (e_s', σ_s')⌝ ∗ state_interp P_t σ_t' P_s σ_s' ∗
+        sim e_t' e_s' Φ)
+
+      ∨ (* call case *)
+      (∃ f K_t v_t K_s v_s σ_s', ⌜e_t = fill K_t (of_call f v_t)⌝ ∗
+        ⌜rtc (prim_step P_s) (e_s, σ_s) (fill K_s (of_call f v_s), σ_s')⌝ ∗
+        val_rel v_t v_s ∗ state_interp P_t σ_t P_s σ_s' ∗
+        sim_ectx K_t K_s Φ)
+    )%I.
+  Proof.
+    by rewrite /sim_ectx !sim_nostutter_eq /uncurry sim_nostutter_def_unfold /step_nostutter.
+  Qed.
+
+  Lemma sim_nostutter_coind Φ (Ψ : exprO → exprO → PROP):
+    Proper ((≡) ==> (≡) ==> (≡)) Ψ →
+    (□ ∀ e_t e_s, Ψ e_t e_s -∗ step_nostutter Φ (λ '(e_s', e_t'), Ψ e_t' e_s') (e_s, e_t)) -∗
+    (∀ e_t e_s, Ψ e_t e_s -∗ e_t ⪯ e_s {{ Φ }}).
+  Proof.
+    iIntros (Hp) "#IH". iIntros (e_t e_s) "H".
+    rewrite sim_nostutter_eq /sim_nostutter_def.
+    set (Ψ_curry := (λ '(e_t, e_s), Ψ e_s e_t)).
+    assert (NonExpansive Ψ_curry) as Hne.
+    { intros ? [e1 e2] [e1' e2'] [H1 H2]. rewrite /Ψ_curry. cbn in H1, H2.
+      apply equiv_dist, Hp.
+      - by apply (discrete_iff _ _) in H1.
+      - by apply (discrete_iff _ _) in H2.
+    }
+
+    iApply (greatest_fixpoint_coind (step_nostutter Φ) Ψ_curry with "[]").
+    { iModIntro. iIntros ([e_s' e_t']) "H'". by iApply "IH". }
+    iApply "H".
+  Qed.
+
+  Global Instance sim_nostutter_proper :
+    Proper (eq ==> eq ==>
+      (pointwise_relation (val Λ) (pointwise_relation (val Λ) (≡))) ==> (≡)) sim.
+  Proof.
+    intros e e' -> e1 e1' -> p1 p2 Heq2.
+    rewrite !sim_nostutter_eq. apply greatest_fixpoint_proper; solve_proper.
+  Qed.
+
+  Lemma sim_nostutter_value Φ v_t v_s :
+    ⊢ Φ v_t v_s -∗ (of_val v_t) ⪯ (of_val v_s) {{ Φ }}.
+  Proof.
+    iIntros "Hv". rewrite sim_nostutter_unfold. iIntros (????) "[Hstate Hreach]".
+    iModIntro. iLeft. iExists (v_t), (v_s), (σ_s). iFrame.
+    iSplitL; first by rewrite to_of_val. eauto.
+  Qed.
+
+  Lemma sim_nostutter_call P_t P_s v_t v_s K_t K_s f Φ :
+    P_t !! f = Some K_t →
+    P_s !! f = Some K_s →
+    progs_are P_t P_s -∗
+    val_rel v_t v_s -∗
+    sim_ectx K_t K_s Φ -∗
+    (of_call f v_t) ⪯ (of_call f v_s) {{ Φ }}.
+  Proof.
+    intros Htgt Hsrc. iIntros "#Prog Val Sim".
+    rewrite sim_nostutter_unfold. iIntros (P_t' σ_t P_s' σ_s) "[SI %]".
+    iModIntro. iRight. iLeft.
+    rewrite /progs_are; iDestruct ("Prog" with "SI") as "[% %]"; subst P_t' P_s'; iClear "Prog".
+    iSplit.
+    - iPureIntro. eapply head_prim_reducible. eexists _, _. by eapply call_head_step_intro.
+    - iIntros (e_t' σ_t' Hstep). iModIntro.
+     pose proof (prim_step_call_inv P_t empty_ectx f v_t e_t' σ_t σ_t') as (K_t' & Heq & -> & ->);
+      first by rewrite fill_empty.
+      rewrite fill_empty in Hstep.
+      iExists _, _; iFrame; iSplit.
+      + iPureIntro. eapply tc_once, head_prim_step, call_head_step_intro, Hsrc.
+      + rewrite fill_empty; assert (K_t' = K_t) as -> by naive_solver. iApply ("Sim" with "Val").
+  Qed.
+
+  Lemma bupd_sim_nostutter Φ e_t e_s :
+    ⊢ (|==> e_t ⪯ e_s {{Φ}}) -∗ e_t ⪯ e_s {{ Φ }}.
+  Proof.
+    iIntros "Hv". rewrite sim_nostutter_unfold. iIntros (????) "H". iMod "Hv". iApply ("Hv" with "H").
+  Qed.
+
+  Lemma sim_nostutter_mono Φ Φ' :
+    ⊢ (∀ v_t v_s, Φ v_t v_s -∗ Φ' v_t v_s)
+       -∗ ∀ e_s e_t : exprO, e_t ⪯ e_s {{ Φ }} -∗ e_t ⪯ e_s {{ Φ' }}.
+  Proof.
+    iIntros "Hmon".
+    iIntros (e_s e_t) "H".
+    iApply (sim_nostutter_coind Φ' (λ e_t e_s, e_t ⪯ e_s {{ Φ }} ∗ (∀ v_t v_s : val Λ, Φ v_t v_s -∗ Φ' v_t v_s))%I); last by iFrame.
+    iModIntro. clear e_t e_s. iIntros (e_t e_s) "[H Hpost]".
+    rewrite sim_nostutter_eq sim_nostutter_def_unfold.
+    rewrite /step_nostutter.
+    iIntros (????) "Hs". iSpecialize ("H" with "Hs"). iMod "H". iModIntro.
+    iDestruct "H" as "[Hval | [Hred | Hcall]]".
+    - iLeft. iDestruct "Hval" as (v_t v_s σ_s') "(?&?&?&?)". iExists v_t, v_s, σ_s'. iFrame. by iApply "Hpost".
+    - iRight; iLeft. iDestruct "Hred" as "[Hred Hstep]". iFrame.
+    - iRight; iRight. iFrame.
+  Qed.
+
+  (* TODO: currently just copied and adapted from the full lemma above; we don't need the factorisation for this simpler simulation *)
+  Definition bind_pred_nostutter Φ := uncurry (λ '(e_s, e_t), ∃ e_t' e_s' (K_t K_s : ectx Λ),
+    ⌜e_t = fill K_t e_t'⌝ ∧ ⌜e_s = fill K_s e_s'⌝ ∧
+     e_t' ⪯ e_s' {{λ v_t v_s : val Λ, fill K_t (of_val v_t) ⪯ fill K_s (of_val v_s) {{Φ}}}})%I.
+
+  (* Lemma used two times in the proof of the bind lemma (for the value cases of the inner and outer induction) *)
+  Lemma sim_bind_val_nostutter P_s e_s σ_s v_s σ_s' e_t v_t K_t σ_t P_t K_s Φ:
+      rtc (prim_step P_s) (e_s, σ_s) (of_val v_s, σ_s') →
+      to_val e_t = Some v_t →
+      (¬ reach_stuck P_s (fill K_s e_s) σ_s) →
+      ⊢ fill K_t (of_val v_t) ⪯ fill K_s (of_val v_s) {{Φ}} -∗
+        state_interp P_t σ_t P_s σ_s' -∗ |==>
+
+        (* val case *)
+        (∃ (v_t' v_s' : val Λ) σ_s'', ⌜to_val (fill K_t e_t) = Some v_t'⌝ ∗
+          ⌜rtc (prim_step P_s) (fill K_s e_s, σ_s) (of_val v_s', σ_s'')⌝ ∗
+          state_interp P_t σ_t P_s σ_s'' ∗ Φ v_t' v_s')
+
+        ∨ (* red case *)
+         ⌜reducible P_t (fill K_t e_t) σ_t⌝ ∗
+         (∀ e_t' σ_t',
+            ⌜prim_step P_t (fill K_t e_t, σ_t) (e_t', σ_t')⌝ -∗ |==>
+              (∃ e_s' σ_s'',
+               ⌜tc (prim_step P_s) (fill K_s e_s, σ_s) (e_s', σ_s'')⌝ ∗ state_interp P_t σ_t' P_s σ_s'' ∗
+               bind_pred_nostutter Φ e_s' e_t'))
+        ∨ (* call case *)
+          (∃ (f : string) (K_t' : ectx Λ) (v_t' : val Λ) (K_s' : ectx Λ) (v_s' : val Λ) σ_s'',
+            ⌜fill K_t e_t = fill K_t' (of_call f v_t')⌝ ∗
+            ⌜rtc (prim_step P_s) (fill K_s e_s, σ_s) (fill K_s' (of_call f v_s'), σ_s'')⌝ ∗
+            val_rel v_t' v_s' ∗ state_interp P_t σ_t P_s σ_s'' ∗
+            (∀ v_t'' v_s'' : val Λ, val_rel v_t'' v_s'' -∗
+              bind_pred_nostutter Φ (fill K_s' (of_val v_s'')) (fill K_t' (of_val v_t'')))).
+  Proof.
+    (* unfold Hpost to examine the result and combine the two simulation proofs *)
+    iIntros (H0 H Hnreach) "Hpost Hstate".
+    rewrite {1}sim_nostutter_eq {1}sim_nostutter_def_unfold.
+    rewrite {1}/step_nostutter.
+    iMod ("Hpost" with "[Hstate]") as "Hpost".
+    { iFrame. iPureIntro. intros Hstuck.
+      eapply Hnreach, prim_step_rtc_reach_stuck; last done.
+      by apply fill_prim_step_rtc. }
+    iModIntro.
+    iDestruct "Hpost" as "[Hv | [Hstep | Hcall]]".
+    + iLeft. iDestruct "Hv" as (v_t' v_s' σ_s'') "(% & % & Hstate & Hpost)".
+      iExists v_t', v_s', σ_s''. iFrame.
+      iSplitL. { iPureIntro. by rewrite -H1 (of_to_val _ _ H). }
+      iPureIntro. etrans; eauto using fill_prim_step_rtc.
+    + iRight; iLeft. iDestruct "Hstep" as "[% Hstep]". iSplitR "Hstep".
+      { iPureIntro. by rewrite (of_to_val _ _ H) in H1. }
+      iIntros (e_t' σ_t') "%". iMod ("Hstep" with "[]") as "Hstep".
+      { iPureIntro. by rewrite (of_to_val _ _ H). }
+      iDestruct "Hstep" as (e_s' σ_s'') "(%&Hstate& Hrec)".
+      iExists e_s', σ_s''. iFrame. iSplitR.
+      { iPureIntro. eapply tc_rtc_l; by eauto using fill_prim_step_rtc. }
+      cbn. iExists e_t', e_s', empty_ectx, empty_ectx. rewrite !fill_empty.
+      do 2 (iSplitR; first auto).
+      iApply sim_nostutter_mono. 2: { rewrite sim_nostutter_eq. iApply "Hrec". }
+      iIntros (??) "H". rewrite !fill_empty.
+      by iApply sim_nostutter_value.
+    + iDestruct "Hcall" as (f K_t' v_t' K_s' v_s' σ_s'') "(%&%&Hvrel&Hstate&Hcall)".
+      (* CA on the reduction of fill K_s v_s to fill K_s' (f v_s') to see if we need to take a step or do the call *)
+      iRight; iRight.
+      iExists f, K_t', v_t', K_s', v_s', σ_s''. iFrame.
+      iSplitR. { iPureIntro. by rewrite -H1 (of_to_val _ _ H). }
+      iSplitR. { iPureIntro. etrans; by eauto using fill_prim_step_rtc. }
+      iIntros (v_t'' v_s'') "Hvrel". cbn.
+      iExists (fill K_t' (of_val v_t'')), (fill K_s' (of_val v_s'')), empty_ectx, empty_ectx.
+      rewrite !fill_empty. do 2 (iSplitR; first auto).
+      iApply sim_nostutter_mono; first last.
+      { rewrite sim_nostutter_eq. by iApply "Hcall". }
+      iIntros (??) "H". rewrite !fill_empty. by iApply sim_nostutter_value.
+  Qed.
+
+  Lemma sim_nostutter_bind e_t e_s K_t K_s Φ:
+    ⊢ e_t ⪯ e_s {{λ v_t v_s : val Λ, fill K_t (of_val v_t) ⪯ fill K_s (of_val v_s) {{Φ}} }}
+      -∗ fill K_t e_t ⪯ fill K_s e_s {{Φ}}.
+  Proof.
+    iIntros "H".
+    iApply (sim_nostutter_coind Φ (λ e_t' e_s', bind_pred_nostutter Φ e_s' e_t')%I).
+    2: { iExists e_t, e_s, K_t, K_s. iFrame. eauto. }
+    iModIntro. clear e_t e_s K_t K_s.
+    iIntros (e_t' e_s') "IH".
+    iDestruct "IH" as (e_t e_s K_t K_s) "[-> [-> H]]".
+    rewrite {1}sim_nostutter_eq {1}sim_nostutter_def_unfold.
+    rewrite /step_nostutter.
+
+    iIntros (????) "[Hs %]". rename H into Hnreach.
+    iMod ("H" with "[Hs]") as "H".
+    { iFrame. iPureIntro. contradict Hnreach. by apply fill_reach_stuck. }
+    iDestruct "H" as "[Hval | [Hstep | Hcall]]".
+    - iDestruct "Hval" as (v_t v_s σ_s') "(%& %&Hstate&Hpost)".
+      by iApply (sim_bind_val_nostutter with "[Hpost] [Hstate]").
+    - (* simply thread through everything *)
+      iModIntro. iRight; iLeft. iDestruct "Hstep" as "[% Hstep]".
+      iSplitR. { iPureIntro. by apply fill_reducible. }
+      iIntros (e_t' σ_t') "%".
+      destruct (fill_reducible_prim_step _ _ _ _ _ _ H H0) as (e_t'' & -> & H1).
+      iMod ("Hstep" with "[]") as "Hstep". { iPureIntro. apply H1. }
+      iModIntro.
+      iDestruct "Hstep" as (e_s' σ_s') "(% & Hstate & Hrec)".
+      iExists (fill K_s e_s'), σ_s'. iFrame. iSplitR.
+      { iPureIntro. by apply fill_prim_step_tc. }
+      cbn. iExists e_t'', e_s', K_t, K_s.
+      do 2 (iSplitR; first auto).
+      rewrite sim_nostutter_eq. iApply "Hrec".
+    - (* simply thread through everything *)
+      iModIntro. iRight; iRight.
+      iDestruct "Hcall" as (f K_t' v_t K_s' v_s σ_s') "(-> & % & Hval & Hstate & Hrec)".
+      iExists f, (comp_ectx K_t K_t'), v_t, (comp_ectx K_s K_s'), v_s, σ_s'.
+      iSplitR; first by rewrite fill_comp.
+      iSplitR. { iPureIntro. rewrite -fill_comp. by apply fill_prim_step_rtc. }
+      iFrame.
+      iIntros (v_t' v_s') "Hv". iSpecialize ("Hrec" with "Hv"). cbn.
+      iExists (fill K_t' (of_val v_t')), (fill K_s' (of_val v_s')), K_t, K_s.
+      iSplitR; first by rewrite -fill_comp. iSplitR; first by rewrite -fill_comp.
+      rewrite sim_nostutter_eq. iApply "Hrec".
+  Qed.
+
+End fix_lang.
+
